add

theories/syntax.v
@@ -7,17 +7,25 @@ Require Import Paco.paco.
 Require Import Coq.btauto.Btauto.
 Require Import ConstructiveEpsilon.
 
-From Containment Require Import  utils.
-
-Check Fix.
-
+From Containment Require Import  utils dsl dsl_theory.
+Set Implicit Arguments.
+Set Maximal Implicit Insertion.
 
 
 Let inE := utils.inE.
 
 Section Regex.
-Variable (A : finType).
+Variable A : finType. (**)
+(*Variable (As : Set).
+Hypothesis (H : Finite.axioms_ As).
+Definition A : finType := @Finite.Pack As H.
+Check @Finite.Pack.
+Check (Finite.sort A).
+Check A.*)
 Definition trace := seq A.
+
+Check nat_rect.
+
 
 Inductive regex : Type :=
 | Eps : regex
@@ -27,15 +35,27 @@ Inductive regex : Type :=
 | Seq : regex -> regex -> regex
 | Star : regex -> regex.
 
-
-(*Notation "e _._ c" := (Seq (Event e) c)
-                    (at level 51, right associativity).*)
-
 Notation "c0 _;_ c1"  := (Seq c0 c1)
                          (at level 52, left associativity).
 
 Notation "c0 _+_ c1"  := (Plus c0 c1)
                          (at level 53, left associativity).
+
+(*Inductive pTree : regex -> Type := 
+| p_tt : pTree Eps 
+| p_singl a : pTree (Event a)
+| p_inl {r0 r1} : pTree r0 -> pTree (r0 _+_ r1) 
+| p_inr r0 r1 : pTree r1 -> pTree (r0 _+_ r1) 
+| p_pair r0 r1 : pTree r0 -> pTree r1 -> pTree (r0 _;_ r1)
+| p_fold r : pTree (Eps _+_ (r _;_ (Star r))) -> pTree (Star r).
+End Regex.
+*)
+
+
+(*Notation "e _._ c" := (Seq (Event e) c)
+                    (at level 51, right associativity).*)
+
+
 
 Definition regex_indDef := [indDef for regex_rect].
 Canonical regex_indType := IndType regex regex_indDef.
@@ -662,12 +682,225 @@ Section parseTrees.
 
 Inductive upTree : Type := 
 | up_tt : upTree
+| up_bot : upTree
 | up_singl (a : A) : upTree
 | up_inl : upTree -> upTree
 | up_inr  : upTree -> upTree
 | up_pair  : upTree -> upTree -> upTree
 | up_fold : upTree  -> upTree.
 
+Check upTree_rect.
+
+Fixpoint upTree_size p := 
+match p with 
+| up_tt =>  1 
+| up_bot => 1 
+| up_singl _ => 1
+| up_inl p0 => (upTree_size p0).+1
+| up_inr p0 => (upTree_size p0).+1
+| up_pair p0 p1=> ((upTree_size p0) + (upTree_size p1)).+1
+| up_fold p0 => (upTree_size p0).+1
+end.
+(*
+Fixpoint take_fix_fuel n (f : (upTree -> upTree) -> upTree -> upTree) : (upTree -> upTree) :=
+if n is n'.+1 then
+ f (take_fix_fuel n' f)
+else id.
+
+Fixpoint take_fix_fuel2 n (f : upTree -> (upTree -> upTree) -> upTree) : (upTree -> upTree) :=
+fun T =>
+if n is n'.+1 then
+ f T (take_fix_fuel2 n' f)
+else T.
+
+Fixpoint take_fix_fuel3 n (p : upTree) (f : upTree -> (upTree -> upTree) -> upTree) : upTree :=
+if n is n'.+1 then
+ f p (fun p' => take_fix_fuel3 n' p' f)
+else p.
+
+
+Definition test_f : upTree -> (upTree -> upTree) -> upTree := 
+fun T f => 
+match T with 
+| up_pair T0 T1 => up_pair T0 (up_pair up_bot (f T1))
+| _ => T
+end.
+
+(*Eval compute in (take_fix_fuel3 0 (up_pair up_tt up_tt) test_f).
+Eval compute in (take_fix_fuel3 1 (up_pair up_tt up_tt) test_f).
+Eval compute in (take_fix_fuel3 2 (up_pair up_tt up_tt) test_f).
+Eval compute in (take_fix_fuel2 2 test_f (up_pair up_tt up_tt)). *)
+
+
+
+Definition pRel (p' p : upTree) := upTree_size p' < upTree_size p.
+
+Definition higher_n (n : nat) := (forall p', upTree_size p' < n -> upTree) -> upTree -> upTree.
+
+Inductive D_fix (n : nat) : higher_n n -> Prop :=
+| D_next n n' f : n' < n -> D_fix f  -> D_fix f.
+
+
+Check @Acc_rect.
+Check (@Acc_rect upTree pRel (fun p => (forall p', pRel p' p -> upTree) -> upTree -> upTree)).
+
+Check upTree_rect.
+
+Lemma upTree_size1 : forall p, 0 < upTree_size p.
+Proof.
+elim=>//.
+Qed.
+
+
+(*Lemma Acc_pRel :  forall p, Acc pRel p.
+Proof. 
+move=> p. move Heq : (upTree_size p)=>n. elim: n p Heq.
+case=>//. move=> n IH. case;intros. con;intros. 
+move: H. rewrite /pRel. simpl.  move: (upTree_size1 y). lia.
+con. intros. move: H. rewrite /pRel. simpl. move: (upTree_size1 y). lia.
+con. intros. move: H. rewrite /pRel. simpl. move: (upTree_size1 y). lia.
+move: Heq. simpl. case. intro. 
+con. intros. apply/IH.
+intros. apply/IH.
+intros.
+rewrite /pRel //=.
+inv H.
+
+simpl. simpl. repeat simpl.
+con. move=> y.*)
+
+Lemma upTree_size_rect
+     : forall P : upTree -> Type,
+       (forall u  : upTree, (forall u', pRel u' u -> P u') -> P u) ->
+       forall u : upTree, P u.
+Proof.
+move=> P Hsize u. 
+have: Acc pRel u. clear Hsize. 
+move Heq : (upTree_size u)=>n. move: n Heq.
+suff : forall n : nat, upTree_size u <= n -> Acc (fun p' p : upTree => pRel p' p) u.
+intros. eauto.
+move=>n. elim: n u.
+intros. con. intros. rewrite /pRel in H0. lia.
+intros. con. intros. apply/H. rewrite /pRel in H1. lia.
+move=>Hacc.
+move: u Hacc Hsize. apply: Acc_rect.
+intros.  apply/Hsize. intros. apply/X. done.
+auto.
+Defined.
+
+Definition my_fix (f : (forall u, (forall u' : upTree, pRel u' u -> upTree) -> upTree)) :  upTree -> upTree:=
+(upTree_size_rect (fun _ => upTree) f).
+
+Lemma sum_bool p p' :  {pRel p p'} + { ~ pRel p p'}.
+Proof. rewrite /pRel. case Heq : (_ <_)=>//. con. done. right. intro. done.
+Defined.
+
+Definition test u : (forall u' : upTree, pRel u' u -> upTree) -> upTree  := 
+fun f => match u with 
+       | up_pair u0 u1 => match sum_bool u0 u with 
+                          | left p => f _ p
+                          | right p => u
+                          end
+       | _ => u
+       end.
+
+Fixpoint interp d (f : (forall u, (forall u' : upTree, pRel u' u -> upTree) -> upTree)) :  upTree -> upTree  := 
+match d with 
+| cfix d' => my_fix (interp d')
+| cguard (var_dsl 0) => 
+
+
+Definition myP (p : upTree) :=  (forall p', pRel p' p -> upTree) -> upTree.
+
+Definition guarded_fun u := (forall u' : upTree, pRel u' u -> upTree) -> upTree.
+
+
+
+
+
+Definition take_my_fix2  (f : forall p, (forall p', pRel p' p -> upTree) -> upTree) : upTree -> upTree := 
+fun T => fix my_fix (H : D_fix (f) {struct H} := f (my_fix (proj H))
+
+
+f (take_mu_fix2 f)
+
+ f p (fun p' => take_fix_fuel3 n' p' f)
+
+Fixpoint take_my_fix (p : upTree) (f : (forall p', pRel p' p -> upTree) -> upTree -> upTree) {struct p} : upTree -> upTree.
+refine ( f (take_my_fix _ f)).
+ f p (fun p' => take_fix_fuel3 n' p' f)
+
+Fixpoint take_fix_fuel11 (p : upTree) (f : (upTree -> upTree) -> upTree -> upTree) (H : D_fix f p) {struct H} : upTree :=
+ f p (fun p' => take_fix_fuel3 n' p' f)
+
+Fixpoint take_fix_fuel22 (p : upTree) (f : upTree -> (upTree -> upTree) -> upTree) (H : D_fix f p) {struct H} : upTree :=
+ f p (fun p' => take_fix_fuel3 n' p' f)
+
+Fixpoint take_fix_fuel3 (p : upTree) (f : upTree -> (upTree -> upTree) -> upTree) (H : D_fix p) {struct H} : upTree :=
+ f p (fun p' => take_fix_fuel3 n' p' f)
+
+ f p (take_fix_fuel3 f)
+
+Eval compute in (take_fix_fuel3 0 (up_pair up_tt up_tt) test_f).
+Eval compute in (take_fix_fuel3 1 (up_pair up_tt up_tt) test_f).
+Eval compute in (take_fix_fuel3 2 (up_pair up_tt up_tt) test_f).
+Eval compute in (take_fix_fuel2 2 test_f (up_pair up_tt up_tt)). 
+
+
+Eval compute in (take_fix_fuel3 4 (up_pair up_tt up_tt) test_f).
+
+
+Fixpoint take_fix_fuel2 (f : forall p, (forall p', pRel p' p -> upTree) -> upTree) : (upTree -> upTree).
+
+
+Fixpoint take_fix_fuel n (f : (upTree -> upTree) -> upTree -> upTree) : (upTree -> upTree) :=
+
+
+ (f : forall p', upTree_size p' < upTree_size p -> upTree) : upTree := 
+
+
+Definition take_fix (p : upTree) (f : forall p', upTree_size p' < upTree_size p -> upTree) : upTree := 
+
+
+Section size_eliminator_for_upTree.
+  Variable P : ∀x, 𝔻ns x -> Type.
+
+
+Section eliminator_for_𝔻ns.
+
+  Variable P : ∀x, 𝔻ns x -> Type.
+
+  Hypothesis (HPi : ∀x D1 D2, P x D1 → P x D2)
+             (HP0 : ∀x E, P _ (𝔻ns_tt x E))
+             (HP1 : ∀x E D, P _ D → P _ (𝔻ns_ff x E D)).
+
+  Fixpoint 𝔻ns_rect x D { struct D } : P x D.
+  Proof.
+    case_eq (b x); intros G.
+    + apply HPi with (1 := HP0 _ G).
+    + apply HPi with (1 := HP1 _ G _ (𝔻ns_rect _ (𝜋_𝔻ns D G))).
+  Qed.
+
+End eliminator_for_𝔻ns.
+
+
+
+Lemma test : forall (P : upTree -> Type), (forall p, (forall p', upTree_size p' < upTree_size p -> P p') -> P p) -> forall (p : upTree), P p.
+Proof.
+move=> P Hsize p. move Heq: (upTree_size p) => n. move: n p Heq.
+fix IH 1. 
+case.
+- clear IH. case=>//=. 
+- move=> n p Heq. apply/Hsize.
+  
+case=>//=. 
+
+ Check upTree_rect.
+apply: upTree_rect.
+Check upTree_ind.
+apply: upTree_rect.
+- move=> H.
+*)
 Definition upTree_indDef := [indDef for upTree_rect].
 Canonical upTree_indType := IndType upTree upTree_indDef.
 
@@ -675,7 +908,7 @@ Definition upTree_hasDecEq := [derive hasDecEq for upTree].
 HB.instance Definition _ := upTree_hasDecEq.
 
 
-Inductive typing : upTree -> regex  -> Type := 
+Inductive typing : upTree -> regex  -> Prop := 
 | pt_tt : typing up_tt Eps 
 | pt_singl a : typing (up_singl a) (Event a)
 | pt_inl  r0 r1 p : typing p r0 -> typing (up_inl p) (r0 _+_ r1)
@@ -693,6 +926,7 @@ Arguments pt_fold {r p}.
 Fixpoint typingb (p : upTree) (r : regex) := 
 match p with
 | up_tt => r == Eps 
+| up_bot => false 
 | up_singl a => r == (Event a)
 | up_inl p0 => if r is Plus r0 _ then typingb p0 r0 else false 
 | up_inr p0 => if r is Plus _ r1 then typingb p0 r1 else false 
@@ -719,8 +953,15 @@ move => p r. elim=>//.
 Qed.
 
 
+(*Inductive pTree (r : regex) :  Type := 
+| p_tt : Eps = r -> pTree r
+| p_to : pTree r.
 
-Inductive pTree : regex -> Type := 
+End parseTrees.
+End Regex.
+
+
+Inductive pTree regex : Type := 
 | p_tt : pTree Eps 
 | p_singl a : pTree (Event a)
 | p_inl r0 r1 : pTree r0 -> pTree (r0 _+_ r1) 
@@ -730,10 +971,10 @@ Inductive pTree : regex -> Type :=
 Arguments p_inl {r0 r1}.
 Arguments p_inr {r0 r1}.
 Arguments p_pair {r0 r1}.
-Arguments p_fold {r}.
+Arguments p_fold {r}.*)
 
 
-Fixpoint to_upTree {r : regex} (p : pTree r) : upTree := 
+(*Fixpoint to_upTree {r : regex} (p : pTree r) : upTree := 
 match p with 
 | p_tt => up_tt
 | p_singl a => up_singl a 
@@ -741,15 +982,15 @@ match p with
 | p_inr _ _ p => up_inr (to_upTree p)
 | p_pair _ _ p0 p1 => up_pair (to_upTree p0) (to_upTree p1)
 | p_fold _ p' => up_fold (to_upTree p')
-end.
+end.*)
 
-Lemma typing_to_upTree : forall r (x : pTree r), typing (to_upTree x) r.
+(*Lemma typing_to_upTree : forall r (x : pTree r), typing (to_upTree x) r.
 Proof.
 move=> r. elim=>//=;eauto.
-Qed.
+Qed.*)
 
 
-Fixpoint to_pTree {p : upTree} {r : regex} (H : typing p r) : pTree r := 
+(*Fixpoint to_pTree {p : upTree} {r : regex} (H : typing p r) : pTree r := 
 match H in typing p r return pTree r  with 
 | pt_tt => p_tt
 | pt_singl a => p_singl a 
@@ -768,34 +1009,35 @@ match T with
 | p_inr _ _ T' => flatten T'
 | p_pair _ _ T0 T1 => (flatten T0) ++ (flatten T1)
 | p_fold _ T' => flatten T' 
-end.
+end.*)
 
 Fixpoint uflatten (T : upTree) : seq A := 
 match T with 
 | up_tt => nil 
 | up_singl a => (a :: nil )
+| up_bot => nil
 | up_inl T' => uflatten T'
 | up_inr T' => uflatten T'
 | up_pair T0 T1 => (uflatten T0) ++ (uflatten T1)
 | up_fold T' => uflatten T' 
 end.
 
-Lemma uflatten_to_upTree : forall r (x : pTree r),  uflatten (to_upTree x) = flatten x.
+(*Lemma uflatten_to_upTree : forall r (x : pTree r),  uflatten (to_upTree x) = flatten x.
 Proof.
 move=> r. elim=>//=.
 move=> r0 r1 p Hf p0 Hf1. rewrite Hf Hf1 //.
-Qed.
+Qed.*)
 
-Lemma flatten_to_pTree : forall r (x : upTree) (H: typing x r), flatten (to_pTree H) = uflatten x.
+(* Lemma flatten_to_pTree : forall r (x : upTree) (H: typing x r), flatten (to_pTree H) = uflatten x.
 Proof.
 move=> r x. elim=>//=;eauto;intros.
 rewrite H H0. done.
-Qed.
+Qed.*)
 
 
 
 Definition genF (l : seq upTree) :=
-  (up_tt::(map up_singl (index_enum A)))++
+  (up_tt::up_bot::(map up_singl (index_enum A)))++
   (map up_inl l)++
   (map up_inr l)++
   (map (fun p => up_pair p.1 p.2) (compose l l pair))++
@@ -823,42 +1065,45 @@ Lemma in_gen_upTree : forall (T : upTree), exists n, T \in gen_upTree n.
 Proof.
 elim=>//.
 - exists 1. rewrite /= /genF //= !inE.
-- exists 1. rewrite /= /genF //= !inE. apply/orP. right. rewrite mem_cat. apply/orP. left.
+- exists 1. rewrite /= /genF //= !inE.
+- exists 1. rewrite /= /genF //= !inE. apply/orP. right. 
+  apply/orP. right. 
+  rewrite mem_cat. apply/orP. left.
   apply/map_f. apply/mem_index_enum.
 - move=> u [] x Hin. exists x.+1. rewrite /= mem_cat /genF /= !inE.
-  apply/orP. right. apply/orP. right.
+  apply/orP. right. apply/orP. right. apply/orP. right.
   rewrite !mem_cat. apply/orP. right.
   apply/orP. left. apply/map_f. done.
 - move=> u [] x Hin. exists x.+1. rewrite /= mem_cat /genF /= !inE.
-  apply/orP. right. apply/orP. right.
+  apply/orP. right. apply/orP. right. apply/orP. right.
   rewrite !mem_cat. apply/orP. right.
   apply/orP. right.  apply/orP. left. apply/map_f. done.
 - move=> u [] x Hin u' [] x' Hin'. exists (x + x').+1.
-  rewrite /= mem_cat /genF /=. rewrite !inE. apply/orP. right.
+  rewrite /= mem_cat /genF /=. rewrite !inE. apply/orP. right. apply/orP. right.
   rewrite !mem_cat. apply/orP. right. apply/orP. right.
   apply/orP. right. apply/orP. right. apply/orP. left. 
   apply/mapP. econ.  apply/mem_compose. apply/in_gen_upTree_le. 
   2: {  apply/Hin. } lia. 
   apply/in_gen_upTree_le. 2 : { apply/Hin'. } lia. done.
 - move=> u [] x Hin. exists x.+1. rewrite /= !mem_cat /genF /= !inE.
-  apply/orP. right. apply/orP. right. apply/orP. right.
-  apply/orP. right. apply/orP. right. apply/map_f. done.
+  apply/orP. right. apply/orP. right. apply/orP. right. apply/orP. right.
+  apply/orP. right. apply/map_f. done.
 Qed.
 
+Check flatten.
 
-
-Lemma exists_pTree : forall r s, Match s r -> exists (T : pTree r), flatten T = s.
+Lemma exists_pTree : forall r s, Match s r -> exists (T : upTree), (typingb T r) &&  (uflatten T == s).
 Proof.
 move => r s. elim=>//;eauto.
-- exists p_tt. done.
-- move=> x. exists (p_singl x). done.
+- exists up_tt. done.
+- move=> x. exists (up_singl x). ssa. 
 - move=> s1 c1 s2 c2 HM [] x Hf HM2 [] x' Hf2. 
-  exists (p_pair x x')=>/=. f_equal=>//.
-- move=> s1 c1 c2 HM [] x Hf. exists (p_inl x). done.
-- move=> s1 c1 c2 HM [] x Hf. exists (p_inr x). done.
-- move => c. exists (p_fold (p_inl p_tt)). done.
-- move=> c s1 s2 HM [] x Hf HM2 [] x' Hf'. exists (p_fold (p_inr (p_pair x x')))=>/=. 
-  f_equal=>//.
+  exists (up_pair x x')=>/=. ssa.   rewrite (eqP H0) (eqP H2) //.
+- move=> s1 c1 c2 HM [] x Hf. exists (up_inl x). done.
+- move=> s1 c1 c2 HM [] x Hf. exists (up_inr x). done.
+- move => c. exists (up_fold (up_inl up_tt)). done.
+- move=> c s1 s2 HM [] x Hf HM2 [] x' Hf'. exists (up_fold (up_inr (up_pair x x')))=>/=. 
+  ssa. rewrite (eqP H0) (eqP H2) //.
 Qed.
 
 Lemma has_sig : forall (A : eqType) (f : A -> bool) (l :seq A), has f l -> { a | f a}.
@@ -870,10 +1115,9 @@ Defined.
 
 Lemma Match_exists_n : forall s r, Match s r -> exists n, has (fun x => (typingb x r) && (uflatten x == s)) (gen_upTree n).  
 Proof.
-move=> s r HM. case: (exists_pTree r s HM)=> x Hf.
-case:(in_gen_upTree (to_upTree x))=> x0 Hin. exists x0.
-apply/hasP. exists (to_upTree x). done. apply/andP. con. apply/typingP2. apply/typing_to_upTree.
-rewrite uflatten_to_upTree. apply/eqP=>//.
+move=> s r HM. case: (exists_pTree  HM)=> x Hf.
+case:(in_gen_upTree x)=> x0 Hin. exists x0.
+apply/hasP. exists x. done. apply/andP. con. ssa. ssa. 
 Qed.
 
 (*We use Constructive Epsilon library*)
@@ -884,30 +1128,101 @@ apply: constructive_indefinite_ground_description. instantiate (1 := id). instan
 move=> x. case Hcase: (has _ _)=>//. con. done. right. done.
 apply/Match_exists_n. done.
 Qed.
-
-Lemma Match_pTree : forall r s, Match s r -> { T : pTree r |  flatten T = s}.
+Check typing.
+Print typing.
+Parameter (p : upTree) (r : regex).
+(*Check (typing p r : Prop). *) Print Finite.axioms_.
+Lemma Match_pTree : forall r s, Match s r -> { T : upTree | prod (typingb T r) (uflatten T == s)}.
 Proof.
 move => r s HM.
-move: (Match_sig_n s r HM)=>[]n. move/has_sig=>[] x.
+move: (Match_sig_n  HM)=>[]n. move/has_sig=>[] x.
 case Hcase: (typingb _ _)=>//=.
 move/typingP1 : Hcase=>Ht.
-move/eqP=>Hu. exists (to_pTree Ht). rewrite flatten_to_pTree. done.
+move/eqP=>Hu. exists x. con. apply/typingP2=>//. apply/eqP. done.
 Qed.
-
 End parseTrees.
-Arguments p_inl {r0 r1}.
+(*Arguments p_inl {r0 r1}.
 Arguments p_inr {r0 r1}.
 Arguments p_pair {r0 r1}.
-Arguments p_fold {r}.
+Arguments p_fold {r}.*)
 
 Arguments pt_inl {r0 r1 p}.
 Arguments pt_inr {r0 r1 p}.
 Arguments pt_pair {r0 r1 p0 p1}.
 Arguments pt_fold {r p}.
+Hint Constructors typing.
 
-Section DSL.
+Section Containment.
+  Variable P : regex -> regex -> dsl -> Prop.
+Reserved Notation "c0 <R= c1 ~> p" (at level 63).
+
+(*Tried as much as possible to stay within Henglein & Nielsen's formulation*)
+(*full_unf pf = ... ensures that pf <> pfix f. f
+  With an explicit fix rule, we would need to ensure guardedness*)
+Inductive c_ineq : regex -> regex -> dsl -> Prop :=
+| rule_shuffle c0 c1 c2 pf : full_unf pf = shuffle -> (c0 _+_ c1) _+_ c2 <R= c0 _+_ (c1 _+_ c2) ~> pf (*assoc  + *)
 
 
+| rule_shuffleinv c0 c1 c2 pf : full_unf pf = shuffleinv -> c0 _+_ (c1 _+_ c2)  <R= (c0 _+_ c1) _+_ c2 ~> pf (*assoc +*)
+
+| rule_retag c0 c1 pf: full_unf pf = retag -> c0 _+_ c1 <R= c1 _+_ c0 ~> pf (*comm +*)(*Other direction is redundant*)
+
+| rule_untagL c pf : full_unf pf = untagL -> Empt _+_ c <R= c ~> pf (* + neut r*)
+| rule_untagLinv c pf: full_unf pf = untagLinv -> c <R= Empt _+_ c ~> pf (*Possibly redundant*)
+
+| rule_untag c pf : full_unf pf = untag ->  c _+_ c <R= c ~> pf (*idem*)
+| rule_tagL c d pf : full_unf pf = tagL ->  c <R= c _+_ d ~> pf
+
+| rule_assoc c0 c1 c2 pf : full_unf pf = assoc ->  (c0 _;_ c1) _;_ c2 <R= c0 _;_ (c1 _;_ c2) ~> pf
+| rule_associnv c0 c1 c2 pf : full_unf pf = associnv -> c0 _;_ (c1 _;_ c2) <R=  (c0 _;_ c1) _;_ c2 ~> pf
+
+| rule_swap c pf : full_unf pf = swap -> (c _;_ Eps) <R= (Eps _;_ c) ~> pf (*New rule, from regex as types paper*)
+| rule_swapinv c pf : full_unf pf = swapinv -> (Eps _;_ c) <R= (c _;_ Eps) ~> pf
+
+| rule_proj c pf : full_unf pf = proj -> (Eps _;_ c) <R= c ~> pf
+| rule_projinv c pf : full_unf pf = projinv -> c <R=(Eps _;_ c) ~> pf
+
+| rule_abortR c pf : full_unf pf = abortR ->  c _;_ Empt <R= Empt ~> pf
+| rule_abortRinv c pf : full_unf pf = abortRinv ->  Empt  <R= c _;_ Empt ~> pf
+
+| rule_abortL c pf : full_unf pf = abortL -> Empt _;_ c <R=  Empt ~> pf
+| rule_abortLinv c pf : full_unf pf = abortLinv -> Empt  <R=  Empt _;_ c ~> pf
+
+| rule_distL c0 c1 c2 pf : full_unf pf = distL -> c0 _;_ (c1 _+_ c2) <R= (c0 _;_ c1) _+_ (c0 _;_ c2) ~> pf
+| rule_distLinv c0 c1 c2 pf : full_unf pf = distLinv -> (c0 _;_ c1) _+_ (c0 _;_ c2)  <R=  c0 _;_ (c1 _+_ c2) ~> pf
+
+| rule_distR c0 c1 c2 pf : full_unf pf = distR -> (c0 _+_ c1) _;_ c2 <R= (c0 _;_ c2) _+_ (c1 _;_ c2) ~> pf
+| rule_distRinv c0 c1 c2 pf : full_unf pf = distRinv ->  (c0 _;_ c2) _+_ (c1 _;_ c2)  <R= (c0 _+_ c1) _;_ c2 ~> pf
+
+
+| rule_wrap c pf : full_unf pf = wrap ->  Eps _+_ (c _;_ Star c) <R= Star c ~> pf
+| rule_wrapinv c pf : full_unf pf = wrapinv -> Star c  <R=Eps _+_ (c _;_ Star c) ~> pf
+
+| rule_drop c pf : full_unf pf = drop ->  Star (Eps _+_ c) <R= Star c ~> pf
+| rule_dropinv c pf : full_unf pf = dropinv ->  Star c <R= Star (Eps _+_ c) ~> pf (*Possibly redundant*)
+
+ (*We want to remove inner Eps, so we only keep this one for now*)
+(*Will the other direction be necessary?*)
+(*| ci_star_plus_inv c :  Star c  <R= Star (Eps _+_ c) (*Could possibly be removed but we are studying the computational interpretation of EQ rules*) *)
+
+| rule_cid c pf : full_unf pf = cid ->  c <R= c ~> pf
+
+(*| ci_sym c0 c1 (H: c0 =R=c1) : c1 =R=c0*)
+| rule_ctrans c0 c1 c2 pf p0 p1 : full_unf pf =  ctrans p0 p1 ->  c0 <R=c1 ~> p0 ->  c1 <R=c2 ~> p1 -> c0 <R=c2 ~> pf
+| rule_cplus c0 c0' c1 c1' pf p0 p1 : full_unf pf = cplus p0 p1 ->  c0 <R=c0' ~> p0 -> c1 <R=c1' ~> p1 -> c0 _+_ c1 <R=c0' _+_ c1' ~> pf
+| rule_cseq c0 c0' c1 c1' pf p0 p1 : full_unf pf = cseq p0 p1 ->  c0 <R=c0' ~> p0 -> c1 <R=c1' ~> p1 ->  c0 _;_ c1 <R=c0' _;_ c1' ~> pf
+| rule_cstar c0 c1 pf p : full_unf pf = cstar p ->  c0 <R=c1 ~> p -> Star c0 <R= Star c1 ~> pf  (*new context rule*) 
+(*| rule_cfix r r' (p  : dsl) : r <R= r' ~> p[d (cfix p) .: var_dsl] ->  r <R= r' ~> (cfix p) (*guarded p otherwise unsound*)*)
+| rule_test a r r' pf p : full_unf pf = guard p -> P r r' p -> (Event a) _;_ r <R= (Event a) _;_ r' ~> pf
+ where "c1 <R= c2 ~> p" := (c_ineq c1 c2 p).
+End Containment.
+
+Notation "c0 < ( R ) = c1 ~> p" := (c_ineq R c0 c1 p)(at level 63).
+Definition INEQ c0 c1 p := paco3 c_ineq bot3 c0 c1 p.
+Notation "c0 <C= c1 ~> p" := (INEQ c0 c1 p)(at level 63).
+
+
+(*Section DSL.
 Inductive dsl (R: regex -> regex -> Type) : regex -> regex -> Type := 
 | shuffle A B C : dsl R ((A _+_ B) _+_ C) (A _+_ (B _+_ C))
 | shuffleinv A B C : dsl R (A _+_ (B _+_ C)) ((A _+_ B) _+_ C)
@@ -987,7 +1302,10 @@ Arguments guard {R a A B}.
 
 CoInductive dsl_co : regex -> regex -> Type := 
 | Co_build A B : (dsl dsl_co) A B -> dsl_co A B.
-Arguments Co_build {A B}.
+(*Arguments Co_build {A B}.*)
+
+
+CoFixpoint co_test :=  Co_build (trans shuffle (guard co_test))*)
 
 (*Inductive star (A : Type) := 
 fold_s : (unit + (A * (star A))) -> star A.
@@ -1039,10 +1357,9 @@ match p return pTree r with
 end.*)
 
 (*Notation "c0 <T= c1" := ((pTree c0) -> (pTree c1))(at level 63).
-Notation "c0 <O= c1" := ((pTree c0) -> option (pTree c1))(at level 63).*)
+Notation "c0 <O= c1 ~> p" := ((pTree c0) -> option (pTree c1))(at level 63).*)
 
-(*Set Implicit Arguments.
-Set Maximal Implicit Insertion.*)
+
 (*Print pair.
 
 Print pTree.
@@ -1056,148 +1373,398 @@ Check pTree_rect.
 Require Import Coq.Program.Equality.
 *)
 
+Notation "c0 <T= c1 ~> p" := (forall s, typing s c0 -> typing (p s) c1)(at level 63).
+
+Definition fType :=  upTree -> upTree. 
+Ltac inve H := inversion_clear H;subst;eauto.
+Ltac lt_once := (match goal with 
+                 | [ H : typing _ (_ _+_ _) |- _] => inve H
+                 | [ H : typing _ (_ _;_ _) |- _] => inve H
+                 | [ H : typing _ (Star _) |- _] => inve H
+                 | [ H : typing _ Eps |- _] => inve H
+                 | [ H : typing _ Empt |- _] => inve H
+                 | [ H : typing _ (Event _) |- _] => inve H
+
+                end).
+Ltac lt := cbv;solve[ eauto | intros;repeat lt_once].
 
 (*(A' _+_ B) _+_ C <T= A' _+_ (B _+_ C).*)
-Definition shuffle_i  : upTree -> option upTree := 
+Definition shuffle_i  : fType := 
 fun  T => 
 match T with
-| up_inl (up_inl T') => Some (up_inl T')
-| up_inl (up_inr T') => Some (up_inr (up_inl T'))
-| up_inr T' => Some (up_inr (up_inr T'))
-| _ => None
+| up_inl (up_inl T') => (up_inl T')
+| up_inl (up_inr T') => (up_inr (up_inl T'))
+| up_inr T' =>  (up_inr (up_inr T'))
+| _ => up_bot
 end.
+Lemma shuffle_i_t  : forall A B C,(A _+_ B) _+_ C <T= A _+_ (B _+_ C) ~> shuffle_i.
+Proof. lt. Qed.
 
-Definition shuffleinv_i  :  A _+_ (B _+_ C)  <T= (A _+_ B) _+_ C :=
+
+(* A _+_ (B _+_ C)  <T= (A _+_ B) _+_ C*)
+Definition shuffleinv_i  : fType :=
 fun  T => 
 match T with 
-| up_inl T' => up_inl (up_inl T')
-| p_inr (up_inl T') => up_inl (p_inr T')
-| p_inr (p_inr T') => (p_inr T')
+| up_inl T' => (up_inl (up_inl T'))
+| up_inr (up_inl T') => (up_inl (up_inr T'))
+| up_inr (up_inr T') =>  ((up_inr T'))
+| _ => up_bot
 end.
+Lemma shuffleinv_i_t : forall A B C,   A _+_ (B _+_ C)  <T= (A _+_ B) _+_ C ~> shuffleinv_i.
+Proof. lt. Qed.
 
-Definition retag_i  : A _+_ B <T= B _+_ A :=
+
+(* A _+_ B <T= B _+_ A *)
+Definition retag_i :  fType  :=
 fun T => 
 match T with 
-| p_inl T' => p_inr T' 
-| p_inr T' => p_inl T'
+| up_inl T' => up_inr T' 
+| up_inr T' => up_inl T'
+| _ => up_bot
 end. 
+Lemma retag_i_t : forall A B,  A _+_ B <T= B _+_ A  ~> retag_i.
+Proof. lt. Qed.
 
-Definition untagL_i A : Empt _+_ A <T= A :=
+(*Empt _+_ A <T= A*)
+Definition untagL_i :  fType :=
 fun T => 
 match T with 
-| p_inl T' => match T' with end 
-| p_inr T' => T' 
+| up_inl T' => match T' with | _ => up_bot  end 
+| up_inr T' => T' 
+| _ => up_bot
 end.
+Lemma untagL_i_t : forall A, Empt _+_ A <T= A ~> untagL_i.
+Proof. lt. Qed.
 
-Definition untagLinv_i {A} : A <T= Empt _+_ A :=
-fun T => p_inr T.
+(* A <T= Empt _+_ A*)
+Definition untagLinv_i :  fType :=
+fun T => up_inr T.
+Lemma untagLinv_i_t : forall A,  A <T= Empt _+_ A ~> untagLinv_i.
+Proof. lt. Qed.
 
-Definition untag_i A : A _+_ A <T= A :=
+(*A _+_ A <T= A*)
+Definition untag_i :  fType  :=
 fun T =>
 match T with 
-| p_inl T' => T'
-| p_inr T' => T'
+| up_inl T' => T'
+| up_inr T' => T'
+| _ => up_bot
 end.
+Lemma untag_i_t : forall A, A _+_ A <T= A ~> untag_i.
+Proof. lt. Qed.
 
-Definition tagL_i {A B} :  A <T= (A _+_ B ) := p_inl.
+(* A <T= (A _+_ B ) *)
+Definition tagL_i : fType  := up_inl.
+Lemma tagL_i_t : forall A B,  A <T= (A _+_ B ) ~>tagL_i.
+Proof. lt. Qed.
 
-Definition assoc_i A B C : ((A _;_ B) _;_ C)<T=  (A _;_ (B _;_ C)) := 
-fun T => let: ((T0,T1),T2) := T in (T0,(T1,T2)).
-
-Definition associnv_i A B C : (A _;_ (B _;_ C)) <T=  ((A _;_ B) _;_ C) :=
-fun T => let: (T0,(T1,T2)) := T in ((T0,T1),T2).
-
-Definition swap_i A :  (A _;_ Eps)<T=  (Eps _;_ A) := fun T => (tt,T.1).
-Definition swapinv_i A : (Eps _;_ A) <T= (A _;_ Eps) := fun T => (T.2,tt).
-
-Definition proj_i A : (Eps _;_ A)<T=  A := snd.
-Definition projinv_i {A} : A <T= (Eps _;_ A) := fun T => (tt,T).
-
-Definition abortR_i A : (A _;_ Empt) <T=  Empt := fun T => match T.2 with end.
-Definition abortRinv_i A : Empt  <T=  (A _;_ Empt) := fun T => match T with end.
-
-Definition abortL_i A : (Empt _;_ A) <T=  Empt := fun T => match T.1 with end.
-Definition abortLinv_i A : Empt <T=   (Empt _;_ A) := fun T => match T with end.
-
-Definition distL_i A B C : (A _;_ (B _+_ C)) <T= ((A _;_ B) _+_ (A _;_ C)) := 
-fun T => let: (T0,T1) := T in 
-match T1 with 
-| p_inl T' => p_inl (T0,T')
-| p_inr T' => p_inr (T0,T')
-end.
-Definition distLinv_i A B C :  ((A _;_ B) _+_ (A _;_ C)) <T= (A _;_ (B _+_ C)) :=
+(* ((A _;_ B) _;_ C)<T=  (A _;_ (B _;_ C))*)
+Definition assoc_i : fType := 
 fun T => 
 match T with 
-| p_inl (T0,T1) => (T0,p_inl T1)
-| p_inr (T0,T1) => (T0,p_inr T1)
+| up_pair (up_pair T0 T1) T2 => up_pair T0 (up_pair T1 T2)
+| _ => up_bot 
 end.
+Lemma assoc_i_t : forall A B C, ((A _;_ B) _;_ C)<T=  (A _;_ (B _;_ C)) ~> assoc_i.
+Proof. lt. Qed.
 
-Definition distR_i A B C : ((A _+_ B) _;_ C) <T=  ((A _;_ C) _+_ (B _;_ C)) :=
-fun T => let: (T0,T1) := T in 
+(*(A _;_ (B _;_ C)) <T=  ((A _;_ B) _;_ C)*)
+Definition associnv_i : fType  :=
+fun T => 
+match T with 
+| up_pair T0 (up_pair T1 T2) => up_pair (up_pair T0 T1) T2
+| _ => up_bot
+end.
+Lemma associnv_i_t : forall A B C, (A _;_ (B _;_ C)) <T=  ((A _;_ B) _;_ C) ~> associnv_i.
+Proof. lt. Qed.
+
+(* (A _;_ Eps)<T=  (Eps _;_ A) *)
+Definition swap_i : fType := 
+fun T => 
+match T with 
+| up_pair T0 up_tt => up_pair up_tt T0
+| _ => up_bot 
+end.
+Lemma swap_i_t : forall A,  (A _;_ Eps)<T=  (Eps _;_ A) ~> swap_i.
+Proof. lt. Qed.
+
+(* (Eps _;_ A) <T= (A _;_ Eps)*)
+Definition swapinv_i : fType := 
+fun T => 
+match T with 
+| up_pair up_tt T' => up_pair T' up_tt
+| _ => up_bot
+end.
+Lemma swapinv_i_t : forall A, (Eps _;_ A) <T= (A _;_ Eps) ~> swapinv_i.
+Proof. lt. Qed.
+
+(* (Eps _;_ A)<T=  A*)
+Definition proj_i : fType := 
+fun T => 
+match T with 
+| up_pair up_tt T' => T'
+| _ => up_bot
+end.
+Lemma proj_i_t : forall A, (Eps _;_ A)<T=  A ~> proj_i.
+Proof. lt. Qed.
+
+(* A <T= (Eps _;_ A)*)
+Definition projinv_i : fType := 
+fun T => up_pair up_tt T.
+Lemma projinv_i_t : forall A,  A <T= (Eps _;_ A) ~> projinv_i.
+Proof. lt. Qed.
+
+(*Does this make sense, the domain is empty*)
+(* (A _;_ Empt) <T=  Empt*)
+Definition abortR_i : fType := 
+fun _ => up_bot.
+Lemma abortR_i_t : forall A, (A _;_ Empt) <T=  Empt ~> abortR_i.
+Proof. lt. Qed.
+(*match T with 
+| up_pair T' up_bot => up_bot
+| _ => up_bot
+end. *)
+
+(*Empt  <T=  (A _;_ Empt)*)
+Definition abortRinv_i : fType  := fun _ => up_bot.
+Lemma abortRinv_i_t : forall A, Empt  <T=  (A _;_ Empt) ~> abortRinv_i.
+Proof. lt. Qed.
+(*fun T => 
+match T with end.*)
+
+(* (Empt _;_ A) <T=  Empt*)
+Definition abortL_i : fType := fun _ => up_bot.
+Lemma abortL_i_t : forall A,  (Empt _;_ A) <T=  Empt ~> abortL_i.
+Proof. lt. Qed.
+(*fun T => match T.1 with end.*)
+
+(* Empt <T=   (Empt _;_ A) *)
+Definition abortLinv_i : fType := fun _ => up_bot.
+Lemma abortLinv_i_t : forall A, Empt <T=   (Empt _;_ A) ~>abortLinv_i.
+Proof. lt. Qed.
+(*fun T => match T with end.*)
+
+(*(A _;_ (B _+_ C)) <T= ((A _;_ B) _+_ (A _;_ C))*)
+Definition distL_i : fType := 
+fun T => 
+match T with 
+| up_pair T0 (up_inl T1) => up_inl (up_pair T0 T1)
+| up_pair T0 (up_inr T1) => up_inr (up_pair T0 T1)
+| _ => up_bot 
+end.
+Lemma distL_i_t : forall A B C, (A _;_ (B _+_ C)) <T= ((A _;_ B) _+_ (A _;_ C)) ~>distL_i.
+Proof. lt. Qed.
+
+(* ((A _;_ B) _+_ (A _;_ C)) <T= (A _;_ (B _+_ C))*)
+Definition distLinv_i : fType :=
+fun T => 
+match T with 
+| up_inl (up_pair T0 T1) => up_pair T0 (up_inl T1)
+| up_inr (up_pair T0 T1) => up_pair T0 (up_inr T1)
+| _ => up_bot
+end.
+Lemma distLinv_i_t : forall A B C, ((A _;_ B) _+_ (A _;_ C)) <T= (A _;_ (B _+_ C)) ~>distLinv_i.
+Proof. lt. Qed.
+
+
+(* ((A _+_ B) _;_ C) <T=  ((A _;_ C) _+_ (B _;_ C))*)
+Definition distR_i : fType :=
+fun T => 
+match T with 
+| up_pair (up_inl T') T1 => up_inl (up_pair T' T1)
+| up_pair (up_inr T') T1 => up_inr (up_pair T' T1)
+| _ => up_bot
+end.
+Lemma distR_i_t : forall A B C, ((A _+_ B) _;_ C) <T=  ((A _;_ C) _+_ (B _;_ C)) ~>distR_i.
+Proof. lt. Qed.
+(*let: (T0,T1) := T in 
 match T0 with 
-| p_inl T' => p_inl (T',T1)
-| p_inr T' => p_inr (T',T1)
-end.
-Definition distRinv_i A B C : ((A _;_ C) _+_ (B _;_ C))  <T= ((A _+_ B) _;_ C) :=
+| up_inl T' => up_inl (T',T1)
+| up_inr T' => up_inr (T',T1)
+end.*)
+
+(* ((A _;_ C) _+_ (B _;_ C))  <T= ((A _+_ B) _;_ C) *)
+Definition distRinv_i : fType :=
 fun T => 
 match T with 
-| p_inl (T0,T1) => (p_inl T0,T1)
-| p_inr (T0,T1) => (p_inr T0,T1)
+| up_inl (up_pair T0 T1) => up_pair (up_inl T0) T1
+| up_inr (up_pair T0 T1) => up_pair (up_inr T0) T1
+| _ => up_bot
 end.
+Lemma distRinv_i_t : forall A B C,  ((A _;_ C) _+_ (B _;_ C))  <T= ((A _+_ B) _;_ C) ~>distRinv_i.
+Proof. lt. Qed.
 
-Definition wrap_i A : (Eps _+_ (A _;_ Star A)) <T= (Star A) := fold_s.
+(*(Eps _+_ (A _;_ Star A)) <T= (Star A)*)
+Definition wrap_i : fType  := up_fold.
+Lemma wrap_i_t : forall A,(Eps _+_ (A _;_ Star A)) <T= (Star A) ~>wrap_i.
+Proof. lt. Qed.
 (*fun T => 
 match T with
 | p_inl _ => nil 
 | p_inr (T0,T1) => cons T0 T1
 end.*)
-Definition wrapinv_i A : (Star A) <T= (Eps _+_ (A _;_ Star A)) := unfold_s.
+
+
+(* (Star A) <T= (Eps _+_ (A _;_ Star A))*)
+Definition wrapinv_i : fType := 
+fun T => 
+match T with 
+| up_fold T' => T'
+| _ => up_bot
+end.
+Lemma wrapinv_i_t : forall A, (Star A) <T= (Eps _+_ (A _;_ Star A)) ~>wrapinv_i.
+Proof. lt. Qed.
+
 (*fun T => 
 match T with 
 | nil => p_inl tt
 | cons a T' => p_inr (a,T')
 end.*)
-Fixpoint drop_i A :  (Star (Eps _+_ A)) <T= (Star A) :=
+
+(*(Star (Eps _+_ A)) <T= (Star A) *)
+Definition drop_i : fType  :=
+fix drop_i T := 
+match T with 
+| up_fold T0 => match T0 with 
+               | up_inl up_tt => up_fold (up_inl up_tt)
+               | up_inr T1 => match T1 with 
+                              | up_pair T2 T3 => match T2 with 
+                                                  | up_inl up_tt => drop_i T3
+                                                  | up_inr T4 => up_fold (up_inr (up_pair T4 (drop_i T3)))
+                                                  | _ => up_bot
+                                                 end
+                              | _ => up_bot
+                             end
+               | _ => up_bot
+               end
+| _ => up_bot
+end.
+
+
+(*Need size induction on T*)
+Lemma drop_i_t : forall A, (Star (Eps _+_ A)) <T= (Star A) ~>drop_i.
+Proof.
+move=> r T. move Heq: (upTree_size T) => n. move: Heq. suff: upTree_size T <= n -> typing T (Star (Eps _+_ r)) -> typing (drop_i T) (Star r).
+move=>HH H2. apply/HH. subst. lia.
+move=> Heq.
+move: n T Heq r. elim=>//=.
+case=>//=.
+move=> n IH. case=>//=. lt. lt. lt. lt. lt. lt. 
+move=> u Hsize r0 Ht.  inv Ht. inv H1. inv H2.  eauto. inv H2. inv H4. inv H3. apply/IH. ssa. done.
+con. con. con. done. apply/IH. ssa. lia. done.
+Qed.
+
+(*Lemma test_drop_i_input : forall a, typing 
+    (up_fold (up_inr (up_pair (up_inr (up_singl a)) (up_fold (up_inr (up_pair (up_inl up_tt) (up_fold (up_inl up_tt))))))))
+    (Star (Eps _+_ (Event a))).
+Proof.
+move=> a. repeat con. 
+Qed.
+
+(*Eval compute in (drop_i test).*)
+
+Lemma test_drop_i_output : forall a, typing 
+    (up_fold (up_inr (up_pair (up_singl a) (up_fold (up_inl up_tt)))))
+    (Star ((Event a))).
+Proof.
+move=> a. repeat con. 
+Qed.*)
+(*Test suceeded*)
+
+(*match wrapinv_i T with
+| up_inl _ => wrap_i (up_inl up_tt)
+| up_inr (up_pair (up_inl up_tt) T') => wrap_i (up_inl up_tt)
+| up_inr T0 => match T0 with 
+               | (up_pair (up_inr T1) T2) => wrap_i (up_inr (up_pair T1 (drop_i T2)))
+               | _ => up_bot
+              end
+| _ => up_bot
+end.
+Fixpoint drop_i : fType  :=
 fix drop_i T := 
 match unfold_s T with
-| p_inl _ => fold_s (p_inl tt)
-| p_inr (a,T') => match a with | p_inl tt => fold_s (p_inl tt) | p_inr a' => fold_s (p_inr (a',drop_i T')) end
-end.
+| up_inl _ => fold_s (up_inl tt)
+| up_inr (a,T') => match a with | up_inl tt => fold_s (up_inl tt) | up_inr a' => fold_s (up_inr (a',drop_i T')) end
+end.*)
 
-Definition dropinv_i A : (Star A) <T= (Star (Eps _+_ A)) :=
+(* (Star A) <T= (Star (Eps _+_ A))*)
+Definition dropinv_i : fType :=
 fix dropinv_i T := 
-match unfold_s T with 
-| p_inl _ => fold_s (p_inl tt)
-| p_inr (a,T') => fold_s (p_inr (p_inr a,dropinv_i T'))
+match T with 
+| up_fold T0 => match T0 with 
+                | up_inl up_tt => up_fold (up_inl up_tt)
+                | up_inr T1 => match T1 with 
+                               | up_pair T2 T3 => up_fold (up_inr (up_pair (up_inr T2) (dropinv_i T3)))
+                               | _ => up_bot 
+                              end 
+                | _ => up_bot 
+                end 
+| _ => up_bot 
 end.
+Lemma dropinv_i_t : forall A, (Star A) <T= (Star (Eps _+_ A)) ~> dropinv_i.
+Proof. 
+move=> r T. move Heq: (upTree_size T) => n. move: Heq. suff: upTree_size T <= n ->typing T (Star r) -> typing (dropinv_i T) (Star (Eps _+_ r)).
+move=>HH H2. apply/HH. subst. lia.
+move=> Heq.
+move: n T Heq r. elim=>//=.
+case=>//=.
+move=> n IH. case=>//=. lt. lt. lt. lt. lt. lt. 
+move=> u Hsize r0 Ht.  inv Ht. inv H1. inv H2.  eauto. inv H2. con. con. con. con. done. apply/IH. ssa. lia. eauto.
+Qed.
 
-Definition cid_i {c} : c <T= c := fun x => x.
+(*match unfold_s T with 
+| up_inl _ => fold_s (up_inl tt)
+| up_inr (a,T') => fold_s (up_inr (up_inr a,dropinv_i T'))
+end.*)
+
+(* A <T= A *)
+Definition cid_i : fType := fun x => x.
+Lemma cid_i_t : forall A, A <T= A ~>cid_i.
+Proof. lt. Qed.
 
 
-Definition cseq_i A A' B B'  (f0 : A <T=  A') (f1 : B <T= B') : (A _;_ B) <T= (A' _;_ B') :=
-fun T => let: (T0,T1) := T in (f0 T0, f1 T1).
-
-Definition cstar_i A B (f : A <T= B) : (Star A)  <T= (Star B) := 
-fix cstar_i T := 
-match unfold_s T with 
-| p_inl _ => fold_s (p_inl tt)
-| p_inr (a,T') => fold_s (p_inr (f a,(cstar_i T')))
-end.
-
-Definition ctrans_i A B C (f : A <T=B) (f' :B <T=C) :  A <T=C :=
-f' \o f.
-
-Definition cplus_i A B A' B' (f :  A <T=A' ) (f' :  B <T=B' ) : A _+_ B <T=A' _+_ B' :=
+(* (f0 : A <T=  A') (f1 : B <T= B') : (A _;_ B) <T= (A' _;_ B') *)
+Definition cseq_i (f0 f1 : fType ) : fType :=
 fun T => 
 match T with 
-| p_inl T' => p_inl (f T')
-| p_inr T' => p_inr (f' T')
+| up_pair T0 T1 => up_pair (f0 T0) (f1 T1)
+| _ => up_bot 
+end. 
+Lemma cseq_i_t : forall A A' B B' f0 f1, A <T=  A' ~> f0 -> B <T= B' ~> f1 -> (A _;_ B) <T= (A' _;_ B') ~> (cseq_i f0 f1).
+Proof. lt. Qed.
+(*let: (T0,T1) := T in (f0 T0, f1 T1).*)
+
+(* (f : A <T= B) : (Star A)  <T= (Star B) *)
+(*Definition cstar_i2 (f : fType) : fType := 
+match T with 
+| up_fold *)
+
+(*match unfold_s T with 
+| up_inl _ => fold_s (up_inl tt)
+| up_inr (a,T') => fold_s (up_inr (f a,(cstar_i T')))
+end.*)
+
+(* (f : A <T=B) (f' :B <T=C) :  A <T=C*)
+Definition ctrans_i (f f' : fType) :  fType :=
+f' \o f.
+Lemma ctrans_i_t : forall A B C f f', A <T=B ~> f ->  B <T=C ~>f' ->  A <T=C ~> (ctrans_i f f').
+Proof. lt. Qed.
+
+(* (f :  A <T=A' ) (f' :  B <T=B' ) : A _+_ B <T=A' _+_ B'*)
+Definition cplus_i (f f' :  fType)  : fType :=
+fun T => 
+match T with 
+| up_inl T' => up_inl (f T')
+| up_inr T' => up_inr (f' T')
+| _ => up_bot
 end.
+Lemma cplus_i_t : forall A A' B B' f f', A <T=A' ~> f -> B <T=B'  ~> f'  -> A _+_ B <T=A' _+_ B' ~> (cplus_i f f').
+Proof. lt. Qed.
 
 
 
 
-Definition shuffle_o A B C : (A _+_ B) _+_ C <O= A _+_ (B _+_ C) := Some \o shuffle_i.  
+(*Definition shuffle_o A B C : (A _+_ B) _+_ C <O= A _+_ (B _+_ C) := Some \o shuffle_i.  
 Definition shuffleinv_o A B C :  A _+_ (B _+_ C)  <O= (A _+_ B) _+_ C := Some \o shuffleinv_i.
 
 Definition retag_o A B : A _+_ B <O= B _+_ A := Some \o retag_i.
@@ -1263,10 +1830,969 @@ fun T =>
 match T with 
 | p_inl T' => omap p_inl (f T')
 | p_inr T' => omap p_inr (f' T')
+end.*)
+
+(*(f : A <O= B) : ((Event a) _;_ A) <O= ((Event a) _;_ B)*)
+Definition guard_i (f : fType) : fType := 
+fun T => 
+match T with 
+| up_pair (up_singl a) T' => up_pair (up_singl a) (f T') 
+| _ => up_bot 
+end.
+Lemma guard_i_t : forall a A B f, A <T= B ~> f  -> ((Event a) _;_ A) <T= ((Event a) _;_ B) ~> (guard_i f).
+Proof. lt. Qed.
+
+Hint Resolve shuffle_i_t shuffleinv_i_t retag_i_t untagL_i_t untagLinv_i_t untag_i_t
+             tagL_i_t assoc_i_t associnv_i_t swap_i_t swapinv_i_t proj_i_t projinv_i_t abortR_i_t
+             abortRinv_i_t abortL_i_t abortLinv_i_t distL_i_t distLinv_i_t distR_i_t distRinv_i_t
+             wrap_i_t wrapinv_i_t drop_i_t dropinv_i_t cid_i_t ctrans_i_t cplus_i_t cseq_i_t (*cstar_i_t*) guard_i_t.
+
+(*Definition opt_fType := upTree -> option upTree.*)
+
+Fixpoint event_count (a : upTree) :=
+match a with 
+| up_tt => 0
+| up_bot => 0
+| up_singl _ => 1
+| up_inl a' => event_count a'
+| up_inr a' => event_count a'
+| up_pair a0 a1 => (event_count a0) + (event_count a1)
+| up_fold a0 => event_count a0
 end.
 
-Definition guard_o {a c0 c1} (f : c0 <O= c1) : ((Event a) _;_ c0) <O= ((Event a) _;_ c1) := 
-fun T => let: (a,T') := T in if f T' is Some T'' then Some (a,T'') else None.
+(*
+| shuffle  => shuffle_i
+| shuffleinv => shuffleinv_i
+
+
+| retag => retag_i
+| untagL => untagL_i
+| untagLinv => untagLinv_i
+| untag => untag_i
+| tagL => tagL_i
+
+| assoc    => assoc_i
+| associnv    => associnv_i
+
+| swap  =>  swap_i
+| swapinv  => swapinv_i
+
+| proj  => proj_i
+| projinv  => projinv_i
+
+| abortR  => abortR_i
+| abortRinv  => abortRinv_i
+
+| abortL  => abortL_i
+| abortLinv => abortLinv_i
+
+| distL    => distL_i
+| distLinv    => distLinv_i
+
+| distR    => distR_i
+| distRinv    => distRinv_i
+
+| wrap  => wrap_i
+| wrapinv  => wrapinv_i
+
+| drop  => drop_i 
+| dropinv  => dropinv_i
+| cid => cid_i*)
+
+Definition interp_base d := 
+match d with 
+| shuffle  => Some shuffle_i
+| shuffleinv => Some shuffleinv_i
+
+
+| retag => Some retag_i
+| untagL => Some untagL_i
+| untagLinv => Some untagLinv_i
+| untag => Some untag_i
+| tagL => Some tagL_i
+
+| assoc    => Some assoc_i
+| associnv    => Some associnv_i
+
+| swap  => Some  swap_i
+| swapinv  => Some swapinv_i
+
+| proj  => Some proj_i
+| projinv  => Some projinv_i
+
+| abortR  => Some abortR_i
+| abortRinv  => Some abortRinv_i
+
+| abortL  => Some abortL_i
+| abortLinv => Some abortLinv_i
+
+| distL    => Some distL_i
+| distLinv    => Some distLinv_i
+
+| distR    => Some distR_i
+| distRinv    => Some distRinv_i
+
+| wrap  => Some wrap_i
+| wrapinv  => Some wrapinv_i
+
+| drop  => Some drop_i 
+| dropinv  => Some dropinv_i
+| cid => Some cid_i
+| _ => None
+end.
+
+
+Definition eRel (a' a : upTree) := event_count a' < event_count a.
+
+Definition not_plus (T : upTree ) :=  match T with | up_inl _ | up_inr _ => false | _ => true end.
+Definition not_pair (T : upTree ) :=  match T with | up_pair _ _ => false | _ => true end.
+Definition not_star_rule (T : upTree ) :=  match T with |  (up_fold (up_inl up_tt)) | (up_fold (up_inr (up_pair _ _))) => false | _ => true end.
+Definition not_guard (T : upTree) := match T with | up_pair (up_singl _) _ => false | _ => true end.
+
+Inductive G_interp : dsl -> upTree -> upTree -> Prop := 
+| G_base d f T : interp_base (full_unf d) = Some f -> G_interp d T (f T)
+| G_trans  d d0 d1 T T' T'' : full_unf d = (ctrans d0 d1) -> G_interp d0 T T'' -> G_interp d1 T'' T' -> G_interp d T T'
+| G_plus_l d d0 d1 T T' : full_unf d =  (cplus d0 d1) ->  G_interp d0 T T'  -> G_interp d (up_inl T) (up_inl T')
+| G_plus_r d d0 d1 T T' : full_unf d = (cplus d0 d1) -> G_interp d1 T T'  -> G_interp d (up_inr T) (up_inr T')
+| G_plus_bot d d0 d1 T : full_unf d = (cplus d0 d1) -> not_plus T ->   G_interp d T up_bot
+| G_seq d d0 d1 T0 T1 T0' T1' : full_unf d =  (cseq d0 d1) -> G_interp d0 T0 T0' -> 
+                              G_interp d1 T1 T1' -> G_interp d (up_pair T0 T1) (up_pair T0' T1')
+| G_seq_bot d d0 d1 T : full_unf d =  (cseq d0 d1) -> not_pair T -> G_interp d  T up_bot
+
+| G_star0 d' d : full_unf d' =(cstar d) ->  G_interp d' (up_fold (up_inl up_tt)) (up_fold (up_inl up_tt))
+
+| G_star1 d' d T1 T1' T2 T2' : full_unf d' =  (cstar d) -> G_interp d T1 T1' -> G_interp (cstar d) T2 T2' ->
+              G_interp d' (up_fold (up_inr (up_pair T1 T2)))  (up_fold (up_inr (up_pair T1' T2')))
+| G_star_bot d' d T : full_unf d' =(cstar d) -> not_star_rule T ->  G_interp d' T up_bot
+| G_guard d' d T T' a : full_unf d' = guard d -> G_interp d T T' -> G_interp d' (up_pair (up_singl a) T) (up_pair (up_singl a) T')
+| G_guard_bot d' d T  : full_unf d' = guard d -> not_guard T ->  G_interp d' T up_bot.
+(*| G_fix_bot d' d T  : full_unf d' = cfix d ->  G_interp d' T up_bot.*)
+
+Hint Constructors G_interp.
+
+Lemma G_interp_unf d p p' : G_interp d p p' -> G_interp (full_unf d) p p'.
+Proof.
+elim=>//=;eauto;intros.
+- apply/G_base. rewrite full_unf_idemp. eauto.
+- apply/G_trans.  rewrite full_unf_idemp. eauto. eauto. done. 
+- apply/G_plus_l. rewrite full_unf_idemp //.  eauto. done.
+- apply/G_plus_r. rewrite full_unf_idemp. eauto. done.
+- apply/G_plus_bot. rewrite full_unf_idemp. eauto. done.
+- apply/G_seq. rewrite full_unf_idemp. eauto. done. done.
+- apply/G_seq_bot. rewrite full_unf_idemp. eauto. done.
+- apply/G_star0. rewrite full_unf_idemp. eauto. 
+- apply/G_star1. rewrite full_unf_idemp. eauto.  done. done.
+- apply/G_star_bot. rewrite full_unf_idemp. eauto.  done. 
+- apply/G_guard. rewrite full_unf_idemp. eauto.  done. 
+- apply/G_guard_bot. rewrite full_unf_idemp. eauto.  done. 
+Qed.
+(*Inductive D_dom : dsl -> upTree -> Prop := 
+| D_trans d0 d1 T :  D_dom d0  T -> (forall T', G_interp d0 T T' ->  D_dom d1 T') -> D_dom  (ctrans d0 d1) T
+| D_plus_l d0 d1 T :  D_dom d0 T  -> D_dom  (cplus d0 d1)  (up_inl T)
+| D_plus_r d0 d1 T :  D_dom d1 T  -> D_dom  (cplus d0 d1) (up_inr T)
+| D_seq d0 d1 T0 T1 :  D_dom d0 T0 -> D_dom d1 T1  -> D_dom (cseq d0 d1) (up_pair T0 T1)
+| D_star0 d :  D_dom  (cstar d) (up_fold (up_inl up_tt))
+| D_star1 d T1 T2 :  D_dom d T1 -> D_dom (cstar d) T2 ->
+              D_dom  (cstar d) (up_fold (up_inr (up_pair T1 T2)))
+| D_guard d T a : D_dom d T -> D_dom (guard d) (up_pair (up_singl a) T).*)
+
+
+Inductive D_dom : dsl -> upTree -> Prop := 
+| D_base d f T : interp_base (full_unf d) = Some f -> D_dom d T
+| D_trans d d0 d1 T : full_unf d = ctrans d0 d1 -> 
+                    D_dom d0  T -> (forall T', G_interp d0 T T' ->  D_dom d1 T') -> D_dom d T
+(*| D_trans d d0 d1 T : full_unf d = ctrans d0 d1 -> 
+                    D_dom d0  T -> (forall T',  D_dom d1 T') -> D_dom d T*)
+| D_plus_l d d0 d1 T : full_unf d = (cplus d0 d1) ->  D_dom d0 T  -> D_dom  d (up_inl T)
+| D_plus_r d d0 d1 T : full_unf d = (cplus d0 d1)  -> D_dom d1 T  -> D_dom d (up_inr T)
+| D_plus_bot d d0 d1 T : full_unf d = (cplus d0 d1) -> not_plus T ->   D_dom d T
+
+| D_seq d d0 d1 T0 T1 : full_unf d = (cseq d0 d1) ->  D_dom d0 T0 -> D_dom d1 T1  -> D_dom d (up_pair T0 T1)
+| D_seq_bot d d0 d1 T : full_unf d =  (cseq d0 d1) -> not_pair T -> D_dom d T
+
+| D_star0 d' d : full_unf d' = cstar d ->  D_dom d' (up_fold (up_inl up_tt))
+| D_star1 d' d T1 T2 : full_unf d' =  (cstar d) -> D_dom d T1 -> D_dom (cstar d) T2 ->
+              D_dom d' (up_fold (up_inr (up_pair T1 T2)))
+| D_star_bot d' d T : full_unf d' =(cstar d) -> not_star_rule T ->  D_dom d' T
+| D_guard d' d T a : full_unf d' =  (guard d) ->  D_dom d T -> D_dom d' (up_pair (up_singl a) T)
+| D_guard_bot d' d T  : full_unf d' = guard d -> not_guard T ->  D_dom d' T.
+(*| D_fix_bot d' d T  : full_unf d' = cfix d ->  D_dom d' T.*)
+
+Hint Constructors D_dom.
+
+
+Lemma D_dom_unf d p : D_dom d p -> D_dom (full_unf d) p.
+Proof.
+elim=>//=;eauto;intros.
+- apply/D_base. rewrite full_unf_idemp. eauto.
+- apply/D_trans.  rewrite full_unf_idemp. eauto. done. eauto.
+- apply/D_plus_l. rewrite full_unf_idemp. eauto. done.
+- apply/D_plus_r. rewrite full_unf_idemp. eauto. done.
+- apply/D_plus_bot. rewrite full_unf_idemp. eauto. done.
+- apply/D_seq. rewrite full_unf_idemp. eauto. done. done.
+- apply/D_seq_bot. rewrite full_unf_idemp. eauto. done.
+- apply/D_star0. rewrite full_unf_idemp. eauto. 
+- apply/D_star1. rewrite full_unf_idemp. eauto.  done. done.
+- apply/D_star_bot. rewrite full_unf_idemp. eauto.  done. 
+- apply/D_guard. rewrite full_unf_idemp. eauto.  done. 
+- apply/D_guard_bot. rewrite full_unf_idemp. eauto.  done. 
+Qed.
+
+  
+Definition proj_trans0  d d0 d1 T (Heq : full_unf d = ctrans d0 d1) (D : D_dom d T) : D_dom d0 T.
+Proof. refine(
+match D in D_dom d' T' return full_unf d' = ctrans d0 d1 -> D_dom d0 T' with 
+| D_trans _ _ _ _ Heq' D' _ => fun HQ => _
+| _ => fun HQ => _
+end Heq).
+rewrite HQ in e. inv e.
+rewrite Heq' in HQ. inversion HQ. subst. apply: D'. (*structurally smaller*)
+all : try solve [rewrite e in HQ; inv HQ].
+Defined.
+
+Definition proj_trans1  d d0 d1 T T' (Heq : full_unf d = ctrans d0 d1) (D : D_dom d T) (H : G_interp d0 T T') : 
+  D_dom d1 T'.
+Proof. refine(
+match D in D_dom d' T return full_unf d' = ctrans d0 d1 -> G_interp d0 T T' -> D_dom d1 T' with 
+| D_trans _ _ _ _ Heq' D' _ => fun HQ HG => _
+| _ => fun HQ HG => _
+end Heq H).
+all : try solve [rewrite e in HQ; inv HQ].
+rewrite HQ in e. inv e.
+rewrite Heq' in HQ. inv HQ. apply/d5. done.
+Defined.
+
+Definition proj_inl  d d0 d1 T' T (Heq : full_unf d = cplus d0 d1) (Heq2 : T' = up_inl T) (D : D_dom d T') : D_dom d0 T.
+Proof. refine(
+match D in D_dom d' T' return  full_unf d' = cplus d0 d1 -> T' = up_inl T  ->  D_dom d0 T with 
+| D_plus_l _ _ _ _ Heq' D' => fun HQ TQ => _
+| _ => fun HQ TQ => _
+end  Heq Heq2). 
+all : try solve [rewrite e in HQ; inv HQ].
+rewrite HQ in e. inv e.
+rewrite HQ in Heq'. inv Heq'.  inv TQ.
+Defined.
+
+Definition proj_inr  d d0 d1 T' T (Heq : full_unf d = cplus d0 d1) (Heq2 : T' = up_inr T) (D : D_dom d T') : D_dom d1 T.
+Proof. refine(
+match D in D_dom d' T' return  full_unf d' = cplus d0 d1 -> T' = up_inr T  ->  D_dom d1 T with 
+| D_plus_l _ _ _ _ Heq' D' => fun HQ TQ => _
+| _ => fun HQ TQ => _
+end  Heq Heq2). 
+all : try solve [rewrite e in HQ; inv HQ].
+rewrite HQ in e. inv e.
+rewrite HQ in Heq'. inv Heq'.  inv TQ.
+rewrite e in HQ. inv HQ.
+Defined.
+
+Definition proj_seq1  d d0 d1 T' T0 T1 (Heq : full_unf d = cseq d0 d1) (Heq2 : T' = up_pair T0 T1) (D : D_dom d T') : D_dom d0 T0.
+Proof. refine(
+match D in D_dom d' T' return  full_unf d' = cseq d0 d1 -> T' = up_pair T0 T1  ->  D_dom d0 T0 with 
+| D_plus_l _ _ _ _ Heq' D' => fun HQ TQ => _
+| _ => fun HQ TQ => _
+end  Heq Heq2). 
+all : try solve [rewrite e in HQ; inv HQ].
+rewrite HQ in e. inv e.
+rewrite HQ in Heq'. inv Heq'.  inv TQ.
+rewrite e in HQ. inv HQ.
+Defined.
+
+Definition proj_seq2  d d0 d1 T' T0 T1 (Heq : full_unf d = cseq d0 d1) (Heq2 : T' = up_pair T0 T1) (D : D_dom d T') : D_dom d1 T1.
+Proof. refine(
+match D in D_dom d' T' return  full_unf d' = cseq d0 d1 -> T' = up_pair T0 T1  ->  D_dom d1 T1 with 
+| D_plus_l _ _ _ _ Heq' D' => fun HQ TQ => _
+| _ => fun HQ TQ => _
+end  Heq Heq2). 
+all : try solve [rewrite e in HQ; inv HQ].
+rewrite HQ in e. inv e.
+rewrite HQ in Heq'. inv Heq'.  inv TQ.
+rewrite e in HQ. inv HQ.
+Defined.
+
+Definition proj_cstar1  d d0 T' T0 T1 T2 (Heq : full_unf d = cstar d0) (Heq2 : T' = up_fold T0) (Heq3 : T0  = up_inr (up_pair T1 T2)) (D : D_dom d T') : D_dom d0 T1.
+Proof. refine(
+match D in D_dom d' T' return  full_unf d' = cstar  d0 -> T' = up_fold T0 ->  T0 = (up_inr (up_pair T1 T2))  ->  D_dom d0 T1 with 
+| D_plus_l _ _ _ _ Heq' D' => fun HQ TQ => _
+| _ => fun HQ TQ => _
+end  Heq Heq2 Heq3).
+all : try solve [rewrite e in HQ; inv HQ].
+all: subst.
+rewrite HQ in e. inv e.
+rewrite HQ in Heq'. inv Heq'.  inv TQ.
+rewrite e in HQ. inv HQ.
+Defined.
+
+(*Lemma proj_trans0 : forall d d0 d1 T, full_unf d = ctrans d0 d1 -> D_dom d T -> D_dom d0 T.
+Proof.
+intros. inv H0. rewrite H in H1. inversion H1. subst.
+inv H1. 
+
+ := *)
+(*match H with 
+| D_trans _ _ _ _ Heq Hd Hd' => *)
+
+(*Need to define output with conformity to build third premise of D_trans*)
+
+Definition proj1 {A : Type} (P : A -> Prop) (x : A) (H : {x: A | P x}) : A := 
+match H with 
+| exist x' _ => x' 
+end.
+
+(*Definition cplus_i (T : upTree) : {T' | G_interp d T T'} := 
+match T as T' in T = T' -> _  with 
+| up_inl T0 => *)
+
+
+
+(*Fixpoint interp (r0 r1 : regex) (d : dsl) (T : upTree)  (HI : INEQ r0 r1 d) (HT : typing T r0) {struct T} :  { T' | G_interp d T T' /\ typing T r1}.*)
+
+Lemma D_dom_not_fix : forall d d0 T, full_unf d = cfix d0 -> ~D_dom d T.
+Proof.
+intros. intro. inv H0;subst. all: try solve [rewrite H // in H1]. 
+Qed.
+
+Fixpoint interp d (T : upTree) (D: D_dom d T) {struct D} : { T' | G_interp d T T'}.
+Proof. refine (
+match full_unf d as d' return D_dom d T -> full_unf d = d' -> { T' | G_interp d T T'}   with 
+| ctrans d0 d1 => fun D Heq => match (interp d0 T (proj_trans0 Heq D)) with 
+                             | exist T'' _ => match interp d1 T'' (proj_trans1 Heq D _) with 
+                                               | exist T''' _ => exist _ T''' _
+                                             end
+                            end
+| cplus d0 d1 => fun D Heq => (match T as T' return T = T' -> { T'' | G_interp d T T''}  with 
+                           | up_inl T0 => fun HT => match interp d0 T0 (proj_inl Heq HT D) with 
+                                                  | exist T0' _ =>  exist _ (up_inl T0') _ 
+                                                end
+                           |  up_inr T1 => fun HT => match interp d1 T1 (proj_inr Heq HT D) with 
+                                                  | exist T1' _ => exist _ (up_inr T1') _ 
+                                                 end
+                           | _ => fun HT => exist _ up_bot _ end) Logic.eq_refl
+| cseq  d0 d1  => fun D Heq => (match T as T' return T = T' ->  { T'' | G_interp d T T''}  with 
+                             | up_pair T0 T1 => fun HT => match (interp d0 T0 (proj_seq1 Heq HT D)),(interp d1 T1 (proj_seq2 Heq HT D)) with 
+                                                 | exist T0' _ ,exist T1' _ =>   exist _ (up_pair T0' T1') _
+                                                end
+                             | _ => fun HT => exist _ up_bot _ end) Logic.eq_refl
+| cstar d0 => fun D Heq  => let T0 := (
+                      (fix cstar_i (T' : upTree) (D' : D_dom d T') {struct T'} := 
+                      (match T' as T'' return T' = T'' ->  { T''' | G_interp d T' T'''}  with 
+                      | up_fold T0 => fun HT => 
+                                     (match T0 as T0' return T0 = T0' ->  { T''' | G_interp d T' T'''}  with 
+                                     | up_inl up_tt => fun HT' => exist _ (up_fold (up_inl up_tt)) _
+                                     | up_inr (up_pair T1 T2) => fun HT' => match (interp d0 T1 (proj_cstar1 Heq HT HT' D)), (cstar_i T2 _) with 
+                                                                          | exist T'' _, exist T2' _ => exist _ (up_fold (up_inr (up_pair T'' T2'))) (_)
+                                                                        end
+                                     | _ => fun HT' => exist _ up_bot _
+                                     end) Logic.eq_refl
+                      | _ => fun HT => exist _ up_bot _
+                      end) Logic.eq_refl ) T _)
+                      in match T0  with 
+                          | exist T' _ => exist _ T' _
+                         end
+| guard  d0 => fun D Heq  => match T as T' return T = T' -> { T'' | G_interp d T T'' } with
+                          | up_pair (up_singl a) T0 => fun HT => match interp d0 T0 _ with 
+                                                             | exist T1 _ => exist _ (up_pair (up_singl a) T1) _ 
+                                                             end 
+                          | _ => fun HT => exist _ up_bot _ 
+                         end Logic.eq_refl
+| _ => fun D Heq => match interp_base (full_unf d) as d' return interp_base (full_unf d) = d' ->  { T'' | G_interp d T T'' } with
+                 |  Some f => fun HT => exist _ (f T) _ 
+                 |  _ => fun HT => exist _ up_bot _
+                end Logic.eq_refl
+end D Logic.eq_refl).
+all: try solve [ subst;eauto |
+                 move: (D_dom_unf D);  rewrite Heq; move=>HH; inv HH | 
+                con; rewrite Heq; rewrite Heq in HT; done |
+                rewrite Heq //= in HT].
+(*- move: (D_dom_unf D). rewrite Heq. move=> HH. inv HH. inv H.
+  apply/H1. done. *)
+
+(*- subst. move: (D_dom_unf D). rewrite Heq=>HH. inv HH. inv H0. Guarded.
+- subst. move: (D_dom_unf D). rewrite Heq=>HH. inv HH. inv H0.
+- subst. move: (D_dom_unf D). rewrite Heq=>HH. inv HH. inv H1.
+- subst. move: (D_dom_unf D). rewrite Heq=>HH. inv HH. inv H1.*)
+
+(*- inv g. inv H. apply/G_star0. eauto. inv H.
+  apply/G_star1. eauto. done. done.
+  inv H. apply/G_star_bot. eauto. done.*) 
+- move: (D_dom_not_fix Heq D)=>//. Guarded.
+- subst. inv D. all: try solve[ rewrite Heq // in H].
+  rewrite Heq in H1. ssa. rewrite Heq in H2. inv H2. 
+Unshelve.
+(*apply/G_star_bot *)
+all: try solve [subst; eauto]. 
+rewrite HT' in HT. 
+- move: (D_dom_unf D). rewrite Heq. move=> HH.   subst. inv D'. inv H1. Guarded.
+- subst.  inv D'.   inv H1.
+- subst. apply/G_star1. eauto. done.  simpl in y.
+- move: (G_interp_unf y). rewrite Heq. move=> HH. done.   
+- move: (D_dom_unf D). rewrite Heq. done.
+Qed.
+
+
+
+
+
+Fixpoint interp d (T : upTree) (D: D_dom d T) {struct D} : { T' | G_interp d T T'}.
+Proof. refine (
+match full_unf d as d' return D_dom d T -> full_unf d = d' -> { T' | G_interp d T T'}   with 
+| ctrans d0 d1 => fun D Heq => match (interp d0 T (proj_trans0 Heq D)) with 
+                             | exist T'' _ => match interp d1 T'' (proj_trans1 Heq D _) with 
+                                               | exist T''' _ => exist _ T''' _
+                                             end
+                            end
+| cplus d0 d1 => fun D Heq => (match T as T' return T = T' -> { T'' | G_interp d T T''}  with 
+                           | up_inl T0 => fun HT => match interp d0 T0 (proj_inl Heq HT D) with 
+                                                  | exist T0' _ =>  exist _ (up_inl T0') _ 
+                                                end
+                           |  up_inr T1 => fun HT => match interp d1 T1 (proj_inr Heq HT D) with 
+                                                  | exist T1' _ => exist _ (up_inr T1') _ 
+                                                 end
+                           | _ => fun HT => exist _ up_bot _ end) Logic.eq_refl
+| cseq  d0 d1  => fun D Heq => (match T as T' return T = T' ->  { T'' | G_interp d T T''}  with 
+                             | up_pair T0 T1 => fun HT => match (interp d0 T0 (proj_seq1 Heq HT D)),(interp d1 T1 (proj_seq2 Heq HT D)) with 
+                                                 | exist T0' _ ,exist T1' _ =>   exist _ (up_pair T0' T1') _
+                                                end
+                             | _ => fun HT => exist _ up_bot _ end) Logic.eq_refl
+| cstar d0 => fun D Heq  => let T0 := (
+                      (fix cstar_i (T' : upTree) (D' : D_dom d T') {struct T'} := 
+                      (match T' as T'' return T' = T'' ->  { T''' | G_interp d T' T'''}  with 
+                      | up_fold T0 => fun HT => 
+                                     (match T0 as T0' return T0 = T0' ->  { T''' | G_interp d T' T'''}  with 
+                                     | up_inl up_tt => fun HT' => exist _ (up_fold (up_inl up_tt)) _
+                                     | up_inr (up_pair T1 T2) => fun HT' => match (interp d0 T1 (proj_cstar1 Heq HT HT' D')), (cstar_i T2 _) with 
+                                                                          | exist T'' _, exist T2' _ => exist _ (up_fold (up_inr (up_pair T'' T2'))) (_)
+                                                                        end
+                                     | _ => fun HT' => exist _ up_bot _
+                                     end) Logic.eq_refl
+                      | _ => fun HT => exist _ up_bot _
+                      end) Logic.eq_refl ) T _)
+                      in match T0  with 
+                          | exist T' _ => exist _ T' _
+                         end
+| guard  d0 => fun D Heq  => match T as T' return T = T' -> { T'' | G_interp d T T'' } with
+                          | up_pair (up_singl a) T0 => fun HT => match interp d0 T0 _ with 
+                                                             | exist T1 _ => exist _ (up_pair (up_singl a) T1) _ 
+                                                             end 
+                          | _ => fun HT => exist _ up_bot _ 
+                         end Logic.eq_refl
+| _ => fun D Heq => match interp_base (full_unf d) as d' return interp_base (full_unf d) = d' ->  { T'' | G_interp d T T'' } with
+                 |  Some f => fun HT => exist _ (f T) _ 
+                 |  _ => fun HT => exist _ up_bot _
+                end Logic.eq_refl
+end D Logic.eq_refl).
+all: try solve [ subst;eauto |
+                 move: (D_dom_unf D);  rewrite Heq; move=>HH; inv HH | 
+                con; rewrite Heq; rewrite Heq in HT; done |
+                rewrite Heq //= in HT].
+(*- move: (D_dom_unf D). rewrite Heq. move=> HH. inv HH. inv H.
+  apply/H1. done. *)
+
+(*- subst. move: (D_dom_unf D). rewrite Heq=>HH. inv HH. inv H0. Guarded.
+- subst. move: (D_dom_unf D). rewrite Heq=>HH. inv HH. inv H0.
+- subst. move: (D_dom_unf D). rewrite Heq=>HH. inv HH. inv H1.
+- subst. move: (D_dom_unf D). rewrite Heq=>HH. inv HH. inv H1.*)
+
+(*- inv g. inv H. apply/G_star0. eauto. inv H.
+  apply/G_star1. eauto. done. done.
+  inv H. apply/G_star_bot. eauto. done.*) 
+- move: (D_dom_not_fix Heq D)=>//. Guarded.
+- subst. inv D. all: try solve[ rewrite Heq // in H].
+  rewrite Heq in H1. ssa. rewrite Heq in H2. inv H2. 
+Unshelve.
+(*apply/G_star_bot *)
+all: try solve [subst; eauto]. 
+rewrite HT' in HT. 
+- move: (D_dom_unf D). rewrite Heq. move=> HH.   subst. inv D'. inv H1. Guarded.
+- subst.  inv D'.   inv H1.
+- subst. apply/G_star1. eauto. done.  simpl in y.
+- move: (G_interp_unf y). rewrite Heq. move=> HH. done.   
+- move: (D_dom_unf D). rewrite Heq. done.
+Qed.
+
+
+
+
+
+Definition guard_i (f : fType) : fType := 
+fun T => 
+match T with 
+| up_pair (up_singl a) T' => up_pair (up_singl a) (f T') 
+| _ => up_bot 
+end.
+
+
+Fixpoint interp d (T : upTree) (D: D_dom d T) {struct D} :  { T' | G_interp d T T'}.
+Proof. refine (
+match full_unf d as d' return  full_unf d = d' -> { T' | G_interp d T T'}  with 
+| ctrans d0 d1 => fun Heq => match interp d0 T (proj_trans0 Heq D) with 
+                          | exist T'' _ => exist (interp d1 T'' (proj_trans1 Heq D)) _
+                         end 
+| cplus d0 d1 => fun Heq => (match T as T' return T = T' ->  { T' | G_interp d T T'}  with 
+                           | up_inl T0 => fun HT => exist (up_inl (interp d0 T0 _)) _
+                           | up_inr T1 => fun HT => exist (up_inr (interp d1 T1 _)) _ 
+                           | _ => fun _ => T 
+                         end) Logic.eq_refl
+| cseq  d0 d1  => fun Heq => match T with up_pair T0 T1 => up_pair (interp d0 T0 _) (interp d1 T1 _) | _ => T end 
+| cstar d0 => fun Heq  => (fix cstar_i T' := 
+                      match T' with 
+                      | up_fold T0 => match T0 with 
+                                     | up_inl up_tt => up_fold (up_inl up_tt)
+                                     | up_inr (up_pair T1 T2) => up_fold (up_inr (up_pair (interp d0 T1 _) 
+                                                                                         (cstar_i T2)))
+                                     | _ => up_bot 
+                                     end
+                      | _ => up_bot
+                      end) T
+| guard  d0 => fun D  => guard_i (fun T => interp d0 T _) T
+| _ => fun D => if interp_base d is Some f then f T else T
+end D Logic.eq_refl).
+move: (D_dom_unf D). rewrite Heq. move=>HH. inv HH. inv H. apply/H1.
+apply/
+ intros. inv 
+admit.
+subst.
+move/D_dom_unf: D. rewrite Heq. intros. inv D. inv H0.
+
+admit.
+admit.
+admit.
+admit.
+admit.
+admit.
+admit.
+admit.
+admit.
+admit.
+admit.
+
+
+ admit.
+apply: D_trans. 
+admit.
+eauto.
+
+
+
+
+
+
+Definition cstar_i (f : fType) : fType := 
+
+Lemma cstar_i_t : forall A B f, A <T= B ~> f -> (Star A)  <T= (Star B) ~> (cstar_i f).
+Proof.
+move=> r r' f Hf T. move Heq: (upTree_size T) => n. move: Heq. suff: upTree_size T <= n -> typing T (Star r) -> typing (cstar_i f T) (Star r').
+move=>HH H2. apply/HH. subst. lia.
+move=> Heq.
+move: n T Heq  r r' Hf. elim=>//=.
+case=>//=.
+move=> n IH. case=>//=. lt. lt. lt. lt. lt. lt. 
+move=> u Hsize r0 r1 Himp Ht.  inv Ht. inv H1. inv H2.  eauto. inv H2. con. con. con. apply/Himp. done. apply/IH. ssa. lia. eauto. 
+done.
+Qed.
+
+(*Fixpoint interp_aux (r0 r1 : regex)
+           (d : dsl dsl_co r0 r1)  (f : forall x y, dsl_co x y -> fType ) :  fType :=
+match d with 
+| shuffle _ _ _ => shuffle_i
+| shuffleinv _ _ _ => shuffleinv_i
+
+
+| retag _ _ => retag_i
+| untagL _ => untagL_i
+| untagLinv _=> untagLinv_i
+| untag _=> untag_i
+| tagL _ _=> tagL_i
+
+| assoc _ _ _ => assoc_i
+| associnv _ _ _ => associnv_i
+
+| swap _ =>  swap_i
+| swapinv _ => swapinv_i
+
+| proj _ => proj_i
+| projinv _ => projinv_i
+
+| abortR _ => abortR_i
+| abortRinv _ => abortRinv_i
+
+| abortL _ => abortL_i
+| abortLinv _=> abortLinv_i
+
+| distL _ _ _ => distL_i
+| distLinv _ _ _ => distLinv_i
+
+| distR _ _ _ => distR_i
+| distRinv _ _ _ => distRinv_i
+
+| wrap _ => wrap_i
+| wrapinv _ => wrapinv_i
+
+| drop _ => drop_i 
+| dropinv _ => dropinv_i
+| cid _=> cid_i
+
+| ctrans _ _ _ d0 d1 => ctrans_i (interp_aux d0 f) (interp_aux d1 f)
+| cplus _ _ _ _ d0 d1 => cplus_i (interp_aux d0 f) (interp_aux d1 f)
+
+| cseq _ _ _ _ d0 d1  => cseq_i (interp_aux d0 f) (interp_aux d1 f)
+| cstar _ _ d0 => cstar_i (interp_aux d0 f)
+(*| rule_cfix r r' (p  : dsl R dsl) : dsl R r  r' ~> p[d (cfix p) .: dsl R var_dsl] ->  r  r' ~> (cfix p) (*guarded p otherwise unsound*)*)
+| guard _ _ _ pco => guard_i (f _ _ pco)
+(*| _ => fun _ => up_bot*)
+end.
+*)
+
+
+(*Fixpoint interp (r0 r1 : regex)
+           (d : dsl2 dsl_co r0 r1)  (f : forall x y, dsl_co x y -> x <O= y ) :  r0 <O= r1 :=
+match d in dsl2 _ r0 r1 return (pTree r0) -> option (pTree r1) with 
+| @cid2 _ A => (@cid_o A)
+| @shuffle2 _ A B C => (@shuffle_o A B C)
+| @shuffleinv2 _ A B C => (@shuffleinv_o A B C)
+| @ctrans2 _ A B C d0 d1 => (@ctrans_o A B C) (@interp _ _ d0 f) (@interp _ _ d1 f)
+| @cplus2 _ A B C D d0 d1 => (@cplus_o A B C D (@interp _ _ d0 f)) (@interp _ _ d1 f)
+| @guard2 _ a A B pco => guard_o (f _ _ pco)
+end.*)
+
+Fixpoint interp_n (n : nat) (r0 r1 : regex) (d : dsl_co r0 r1) : fType :=
+match d with 
+| Co_build _ _ dco => if n is n'.+1 then interp_aux dco (@interp_n n') else fun _ => up_bot
+end. 
+
+
+
+
+(*Lemma interp_aux_le : forall r r' (d: dsl dsl_co r r') (f : forall x y, dsl_co x y -> fType) T, 
+(forall x y (d : dsl_co x y) T, upTree_size (f _ _ d T) <= upTree_size T) ->  upTree_size (interp_aux d f T) <= upTree_size T.
+Proof.
+move=> r r' d f T.
+destruct T;ssa.
+destruct d;ssa.
+
+elim: d T=>//=;intros. case: T=>//. move=>u. simpl. destruct u;ssa.
+simpl.
+ elim=>//.
+*)
+(*Lemma interp_aux_ext : forall r0 r1 (d : dsl dsl_co r0 r1) (f f' : forall x y, dsl_co x y -> fType) n T, upTree_size T < n ->
+ ( forall T, upTree_size T < n -> forall x y (d : dsl_co x y), f _ _ d = f' _ _ d) -> interp_aux d f T = interp_aux d f' T. 
+Proof.
+move=> r0 r1. elim=>//.
+- move=> A0 B C d IH d0 IH2 f f' n T Hsize Hext.
+  rewrite /= /ctrans_i /=. erewrite IH. 2 : eauto. apply/IH2.*)
+
+
+(*Lemma interp_n_unf : forall i n r0 r1 (d : dsl_co r0 r1) T, upTree_size T < n -> interp_n n d T = interp_n (i + n) d T. 
+Proof.
+elim=>//.
+move=> n IH n0 r0 r1 d T Hsize /=. destruct d. 
+destruct n0. move:(upTree_size1 T). lia.
+simpl. destruct d=>//.
+rewrite /= /ctrans_i /=. rewrite -IH.
+f_equal.
+rewrite -IH.
+f_equal. 
+rewrite IH //=.
+rewrite /interp_aux.
+*)
+Definition interp (r0 r1 : regex) (d : dsl_co r0 r1) : fType := fun T => interp_n (upTree_size T) d T.
+
+(*Require Import Coq.Program.Equality.*)
+Lemma interp_n_unf_typing : forall r0 r1 (d : dsl dsl_co r0 r1) T (f : forall x y (d' : dsl_co x y), fType), 
+(forall x y (d' : dsl_co x y) T', typing T' x -> typing (f _ _ d' T') y)  ->  typing T r0 -> typing (interp_aux d f T) r1. 
+Proof.
+move=> r0 r1. elim=>//;eauto.
+intros. inve H2. simpl.  eauto.  simpl.  eauto. 
+intros. inve H2. simpl.  eauto. 
+intros. inve H1. simpl. inve H2. inve H1. inve H1. con. con. con. eauto. eauto.
+intros. inve H0. simpl. inve H1. 
+Qed.
+
+(*Lemma interp_aux_cstar : forall T r0 r1 (d : dsl dsl_co r0 r1) (f f' : forall x y (d' : dsl_co x y), fType), typing T r0 ->  
+(forall x y (d' : dsl dsl_co x y) T', typing T' x -> interp_aux d' f T' = interp_aux d' f' T') ->  
+(forall x y (d' : dsl_co x y) T', typing T' x -> typing (f _ _ d' T') y) ->
+interp_aux (cstar d) f T = interp_aux (cstar d) f' T.
+Proof.
+move=> T. move Heq: (upTree_size T)=>n. move: Heq.
+suff:  upTree_size T <= n ->
+  forall (r0 r1 : regex) (d : dsl dsl_co r0 r1)
+    (f f' : forall x y : regex, dsl_co x y -> fType),
+  typing T r0 ->
+ (forall (x y : regex) (d' : dsl dsl_co x y) (T' : upTree), typing T' x -> interp_aux d' f T' = interp_aux d' f' T') ->
+  (forall (x y : regex) (d' : dsl_co x y), x <T= y ~> f x y d') -> interp_aux (cstar d) f T = interp_aux (cstar d) f' T.
+move=>HH H2. intros. apply/HH;eauto. subst. lia.
+move=> Heq.
+move: n T Heq r. elim=>//=.
+case=>//=.
+move=> n IH. case=>//=. 
+move=> u Hsize _ r1 r2 d f f' Ht Heq Hf. inv Ht.   inv H0.  inv H2. 
+
+f_equal. f_equal. f_equal. apply/Heq.  done. admit. apply/IH. ssa. lia. done. eauto. eauto. eauto.
+admit. apply/IH. apply/IH;eauto. ssa. lia.
+lt. lt. lt. lt. lt. lt. 
+move=> u Hsize r0 Ht.  inv Ht. inv H1. inv H2.  eauto. inv H2. inv H4. inv H3. apply/IH. ssa. done.
+con. con. con. done. apply/IH. ssa. lia. done.
+Qed.*)
+
+(*Lemma interp_aux_cstar : forall T r0 r1 (d : dsl dsl_co r0 r1) (f f' : forall x y (d' : dsl_co x y), fType), typing T r0 ->  
+(forall T, typing T d ->  interp_aux d f T = interp_aux d f' T) -> 
+interp_aux (cstar d) f T = interp_aux (cstar d) f' T.
+Proof.
+move=> T. move Heq: (upTree_size T)=>n. move: Heq.
+suff:  upTree_size T <= n ->
+  forall (r0 r1 : regex) (d : dsl dsl_co r0 r1)
+    (f f' : forall x y : regex, dsl_co x y -> fType),
+  typing T r0 ->
+  interp_aux (cstar d) f T = interp_aux (cstar d) f' T.
+move=>HH H2. intros. apply/HH;eauto. subst. lia.
+move=> Heq.
+move: n T Heq r. elim=>//=.
+case=>//=.
+move=> n IH. case=>//=. 
+move=> u Hsize _ r1 r2 d f f' Ht. inv Ht.   inv H0.  inv H2. 
+
+f_equal. f_equal. f_equal. admit. apply/IH. ssa. lia. done. eauto. eauto. eauto.
+admit. apply/IH. apply/IH;eauto. ssa. lia.
+lt. lt. lt. lt. lt. lt. 
+move=> u Hsize r0 Ht.  inv Ht. inv H1. inv H2.  eauto. inv H2. inv H4. inv H3. apply/IH. ssa. done.
+con. con. con. done. apply/IH. ssa. lia. done.
+Qed.
+
+
+elim: n Heq=>//.
+
+
+
+
+Lemma interp_aux_cstar : forall T r0 r1 (d : dsl dsl_co r0 r1) (f f' : forall x y (d' : dsl_co x y), fType), typing T r0 ->  
+(forall x y (d' : dsl_co x y) T', typing T' x -> f _ _ d' T' = f' _ _ d' T') ->  
+(forall x y (d' : dsl_co x y) T', typing T' x -> typing (f _ _ d' T') y) ->
+interp_aux (cstar d) f T = interp_aux (cstar d) f' T.
+Proof.
+move=> T. move Heq: (upTree_size T)=>n. move: Heq.
+suff:  upTree_size T <= n ->
+  forall (r0 r1 : regex) (d : dsl dsl_co r0 r1)
+    (f f' : forall x y : regex, dsl_co x y -> fType),
+  typing T r0 ->
+  (forall (x y : regex) (d' : dsl_co x y) (T' : upTree),
+   typing T' x -> f x y d' T' = f' x y d' T') ->
+  (forall (x y : regex) (d' : dsl_co x y), x <T= y ~> f x y d') ->
+  interp_aux (cstar d) f T = interp_aux (cstar d) f' T.
+move=>HH H2. intros. apply/HH;eauto. subst. lia.
+move=> Heq.
+move: n T Heq r. elim=>//=.
+case=>//=.
+move=> n IH. case=>//=. 
+move=> u Hsize _ r1 r2 d f f' Ht Heq Hf. inv Ht.   inv H0.  inv H2. 
+
+f_equal. f_equal. f_equal. admit. apply/IH. ssa. lia. done. eauto. eauto. eauto.
+admit. apply/IH. apply/IH;eauto. ssa. lia.
+lt. lt. lt. lt. lt. lt. 
+move=> u Hsize r0 Ht.  inv Ht. inv H1. inv H2.  eauto. inv H2. inv H4. inv H3. apply/IH. ssa. done.
+con. con. con. done. apply/IH. ssa. lia. done.
+Qed.
+
+
+elim: n Heq=>//.
+*)
+Lemma interp_n_unf : forall r0 r1 (d : dsl dsl_co r0 r1) T (f f' : forall x y (d' : dsl_co x y), fType), typing T r0 -> 
+(forall x y (d' : dsl_co x y) T', typing T' x -> f _ _ d' T' = f' _ _ d' T') ->  
+(forall x y (d' : dsl_co x y) T', typing T' x -> typing (f _ _ d' T') y) ->
+interp_aux d f T = interp_aux d f' T. 
+Proof.
+move=> r0 r1. elim=>//.
+intros. rewrite /= /ctrans_i /=. erewrite H;eauto. apply/H0;eauto.
+erewrite <- H;eauto. apply/interp_n_unf_typing. eauto. done.
+intros. rewrite /=. rewrite /cplus_i. inve H1. f_equal. eauto. f_equal. eauto.
+intros. rewrite /= /cseq_i /=. inve H1. f_equal. eauto. eauto.
+intros. rewrite /=. inve H0. inv H3. inv H5.
+elim: d H;ssa.
+/cstar_i /=.
+destruct T;ssa. f_equal. apply/H. done.
+erewrite H0.
+intros.
+eauto.
+move=> r0 r1 d T f f' Ht.
+elim: Ht d=>//=.
+- move=> d Hf. dependent induction d;ssa.
+  rewrite /ctrans_i /=.
+dependent destruction d.
+ inv d.
+
+Lemma interpP : forall r0 r1 (d : dsl_co r0 r1) T, upTree_size T < n -> typing T r0 -> typing (interp_n n d T) r1. 
+
+
+Lemma interpP : forall r0 r1 (d : dsl_co r0 r1) T, typing T r0 -> typing (interp d T) r1 /\ uflatten T = (uflatten (interp d T)).
+Proof. Admitted.
+
+(*Lemma interp_uflatten : forall r0 r1 (d : dsl_co r0 r1) T, typing T r0 -> typing (interp d T) r1.*)
+
+
+(*Fixpoint interp_wrap (n : nat) (r0 r1 : regex) (d : dsl_co r0 r1) : r0 <O= r1 :=
+match d in dsl_co x y return x <O= y  with 
+          | Co_build _ _ dco => if n is n'.+1 then interp dco (interp_wrap n') else fun _ => None
+end. *)
+
+
+
+(*Lemma fix_eq : forall n, (fix interp_wrap (n0 : fin) (r0 r1 : regex) (d0 : dsl_co r0 r1) {struct n0} : fType := 
+match d0 in (dsl_co x y) h
+    | @Co_build A1 B0 dco => match n0 with
+                            | 0 => fun=> up_bot
+                            | n'.+1 => interp dco (@interp_wrap n')
+                            end
+ end) n = interp_wrap n.
+Proof. done. Qed.*)
+
+Lemma interp_wrap_unf : forall n r0 r1 (d : dsl_co r0 r1), interp_wrap n.+1 d = match d  with 
+          | Co_build _ _ dco => interp dco (@interp_wrap n) end.
+Proof. move => n r0 r1 d //=. Qed.
+
+
+
+
+
+
+(*Require Import Coq.Program.Equality.*)
+(*Check interp.
+Lemma interp_wrap0 : forall r0 r1 (d : dsl2 dsl_co r0 r1), interp d (interp_wrap 0) = fun _ => None.
+Proof.
+move => r0 r1 d. fext. move=> x. 
+elim: d x=>//.
+rewrite /interp_wrap. case: d=>//.
+Qed.*)
+
+Lemma interp_trans : forall r0 r1 r2  (f : forall x y, dsl_co x y -> fType) (d : dsl dsl_co r0 r1) (d' : dsl dsl_co r1 r2) T, interp (ctrans d d') f T -> interp d f T.
+Proof.
+move=> r0 r1 r2 f d d' T. rewrite /= /ctrans_o /obind /oapp /=. case: (interp _ _ _)=>//.
+Qed.
+
+
+Lemma interp_trans2 : forall r0 r1 r2  (f : forall x y, dsl_co x y -> x <O= y)  (d : dsl2 dsl_co r0 r1) (d' : dsl2 dsl_co r1 r2) T T', interp (ctrans2 d d') f T -> interp d f T = Some T' -> interp d' f T'.
+Proof.
+move => r0 r1 r2 Hf d d' T T' /= + Hsome. rewrite /= /ctrans_o /obind /oapp /=. rewrite Hsome //.
+Qed.
+
+Lemma pTree_eq : forall (A0 : regex), (fix pTree (r : regex) : Type := match r with
+                                           | Eps => unit
+                                           | Empt => void
+                                           | Event a => {a' : A & a' == a}
+                                           | r0 _+_ r1 => (pTree r0 + pTree r1)%type
+                                           | r0 _;_ r1 => (pTree r0 * pTree r1)%type
+                                           | Star r0 => seq (pTree r0)
+                                           end) A0 = pTree A0.
+Proof. done. Qed.
+
+Lemma reg_size1 : forall a (T : pTree (Event a)), @reg_size (Event a) T = 1.
+Proof.
+move=> a T. rewrite /reg_size //.
+Qed.
+
+Lemma interp_ineq : forall A B (d : dsl2 dsl_co A B) (T : pTree A) (T' : pTree B) (f : forall x y, dsl_co x y -> x <O= y), (forall x y (dco : dsl_co x y) (T0 : pTree x) (T1 : pTree y) , f x y dco T0 = Some T1 -> reg_size T1 <= reg_size T0) ->  
+                                                                                                                    interp d f T = Some T' -> reg_size T' <= reg_size T.
+Proof.
+move=> A' B d T T' f Hf.  
+- elim: d T T'.
+ *  move=> B0 T0 T1 /=. rewrite /cid_o. case=>//->//.
+ * move => A0 B0 C T T' /=. rewrite /shuffle_o /shuffle_i /=. case=><-. case: T=>//. by case.
+ * move=> A0 B0 C T T' /=. rewrite /shuffleinv_o /shuffleinv_i /=. case=><-. case: T=>//. by case.
+ * move=> A0 B0 C d IH d0 IH2 T T' Hsome. 
+   have: interp (ctrans2 d d0) f T by rewrite Hsome//. 
+   move/[dup]=>Tsome. move/interp_trans.
+   case Heq: (interp _ _ _)=>// [T''] _. move: (IH _ _ Heq)=>Hsize. 
+   move/interp_trans2: (Heq). move/(_ _ d0 Tsome).
+   case Heq2: (interp _ _ _)=>// [T'''] _. move: (IH2 _ _ Heq2). 
+   move=> Hsize2.
+   move: Hsome. rewrite /= /ctrans_o /= /obind /oapp /= Heq Heq2.
+   case. move=> HT;subst. lia.
+ * move=> A0 B0 C D d IH d0. move=> IH2 T T' /=. rewrite /cplus_o /=. 
+   case: T. 
+  **  move=> T2. rewrite /omap /obind /oapp. 
+      case Heq: (interp _ _ _) => // [T3 ]. case. move=> HT3;subst. apply/IH. eauto. 
+  **  move=> T2. rewrite /omap /obind /oapp. 
+      case Heq: (interp _ _ _) => // [T3 ]. case. move=> HT3;subst. apply/IH2. eauto. 
+ * move => A0 B0 r T T' /= T'0. rewrite /guard_o. destruct T' eqn:Heqn. subst. destruct (f _ _ _ _) eqn:Heqn. case. move=> Ht0;subst. 
+   suff: reg_size a1 <= reg_size a0. lia.  eauto. done.
+Qed.
+Check interp_wrap.
+Lemma interp_wrap_ineq : forall n A B (d : dsl_co A B) (T : pTree A) (T' : pTree B),  interp_wrap n d T = Some T' -> reg_size T' <= reg_size T.
+Proof.
+elim.
+- move=> A0 B [] //=.
+- move=> n IH A0 B [] T T' d T0 T0'. rewrite interp_wrap_unf. move=> Hint.  apply/interp_ineq;last by eauto. 
+  move=> x y dco T1 T2 Hin. eauto.
+Qed.
+
+
+Lemma interp_some : forall A B (f : forall x y, dsl_co x y -> x <O= y) (d : dsl2 dsl_co A B) (T : pTree A) , (forall x y (dco : dsl_co x y) (T0 : pTree x), f x y dco T0) ->  
+                                                                                                                    interp d f T.
+Proof.
+move=> A' B f. 
+- elim=>//. 
+ * move=> A0 B0 C d IH d0 IH2 T Hf. 
+   rewrite /= /ctrans_o /obind /oapp /=.
+   move: (@IH T Hf). case Hcase: (interp _ _ _)=>// [T1] _.
+   apply/IH2. eauto.
+ * move=> A0 B0 C D d IH d0. move=> IH2 T Hf /=. rewrite /cplus_o /=. 
+   case: T. 
+  **  move=> T2. rewrite /omap /obind /oapp. 
+      move: (@IH T2 Hf).
+      case Heq: (interp _ _ _) => // [T3 ]. 
+  **  move=> T2. rewrite /omap /obind /oapp. 
+      move: (@IH2 T2 Hf).
+      case Heq: (interp _ _ _) => // [T3 ]. 
+ * move => A0 B0 C r T Hf /=. rewrite /guard_o. destruct T eqn:Heqn;subst.
+   move: (Hf B0 C r a0). case: (f _ _ _)=>//.
+Qed.
+
+Lemma interp_wrap_some : forall n r0 r1 (d : dsl_co r0 r1) (T : pTree r0), reg_size T < n -> interp_wrap n d T.
+Proof.
+elim.
+- move=> r0 r1 d T // Hsize.  
+- move => n IH r0 r1 d T Hsize /=. destruct d.
+  elim: d T Hsize IH=>//.
+ * move=> A1 B0 C d IH d0 IH2 T Hsize IH3 /=. rewrite /ctrans_o /obind /oapp /=.
+   have: interp d (interp_wrap n) T;first by eauto. case Hcase: (interp _ _ _)=>// [ T1 ] _.
+   apply/IH2.
+   have : reg_size T1 <= reg_size T by 
+   apply/interp_ineq;last eauto; move=> x y dco T0 T2 Hint; apply/interp_wrap_ineq; eauto.
+   move=> Hsize2. lia.
+ * move=> r0 r1 d1 T0. eauto.
+ * move=> A1 B0 C D d IH d0 IH1 T Hsize IH2 /=. rewrite /cplus_o.
+   destruct T; rewrite /omap /obind /oapp.
+   have: interp d (interp_wrap n) a. eauto. case Hcase: (interp _ _ _)=>//.
+   rewrite /omap /obind /oapp.
+   have: interp d0 (interp_wrap n) a. eauto. case Hcase: (interp _ _ _)=>//.
+ * move=> a B0 C r T Hsize IH /=. rewrite /guard_o. destruct T.
+   have: (interp_wrap n r a1). by eauto. case: (interp_wrap _ _ _)=>//.
+Qed.
+
+Lemma interp_wrap_sig : forall n r0 r1 (d : dsl_co r0 r1) (T : pTree r0), reg_size T < n -> { T' | interp_wrap n d T = Some T'}.
+Proof.
+move=> n r0 r1 d T Hsize.
+move: (interp_wrap_some  n d T Hsize). case Hcase: (interp_wrap n d T)=>// [T'] _. econ. eauto.
+Qed.
+
+Lemma size_proof : forall (r : regex) (T : pTree r), leq ((reg_size T)) (reg_size T). done. Defined.
+
+Definition interp_total (r0 r1 : regex) (d : dsl_co r0 r1) := 
+fun T =>
+match interp_wrap_sig (reg_size T).+1 d T (size_proof r0 T) with
+| exist T' _ => T'
+end.
+
+
+
+
+
+
+
+
+
+
+
+
+
+(*let: (a,T') := T in if f T' is Some T'' then Some (a,T'') else None.*)
 
 (*This judgment is redundant and we show why*)
 (*Since dsl is intrinsically typed, there is a 1-to-1 correspondance between derivations in the rules from
@@ -1355,7 +2881,7 @@ Proof.
 elim=>//=;eauto. 
 move=> r IH r0 IH2. move=> Hor. destruct (nu r) eqn:Heqn. eauto. eauto.
 move => r IH r0 IH2. move/andP. case. intros. eauto.
-Qed.
+Qed. 
 
 Definition nu_pTree (r : regex) (H : nu r) : (pTree r).
 move: (to_Nu _ H). clear H.
@@ -1483,72 +3009,6 @@ end.
 
 
 
-(*Tried as much as possible to stay within Henglein & Nielsen's formulation*)
-(*full_unf pf = ... ensures that pf <> pfix f. f
-  With an explicit fix rule, we would need to ensure guardedness*)
-Inductive c_ineq : regex -> regex -> dsl -> Prop :=
-| rule_shuffle c0 c1 c2 pf : full_unf pf = shuffle -> (c0 _+_ c1) _+_ c2 <R= c0 _+_ (c1 _+_ c2) ~> pf (*assoc  + *)
-
-
-| rule_shuffleinv c0 c1 c2 pf : full_unf pf = shuffleinv -> c0 _+_ (c1 _+_ c2)  <R= (c0 _+_ c1) _+_ c2 ~> pf (*assoc +*)
-
-| rule_retag c0 c1 pf: full_unf pf = retag -> c0 _+_ c1 <R= c1 _+_ c0 ~> pf (*comm +*)(*Other direction is redundant*)
-
-| rule_untagL c pf : full_unf pf = untagL -> Empt _+_ c <R= c ~> pf (* + neut r*)
-| rule_untagLinv c pf: full_unf pf = untagLinv -> c <R= Empt _+_ c ~> pf (*Possibly redundant*)
-
-| rule_untag c pf : full_unf pf = untag ->  c _+_ c <R= c ~> pf (*idem*)
-| rule_tagL c d pf : full_unf pf = tagL ->  c <R= c _+_ d ~> pf
-
-| rule_assoc c0 c1 c2 pf : full_unf pf = assoc ->  (c0 _;_ c1) _;_ c2 <R= c0 _;_ (c1 _;_ c2) ~> pf
-| rule_associnv c0 c1 c2 pf : full_unf pf = associnv -> c0 _;_ (c1 _;_ c2) <R=  (c0 _;_ c1) _;_ c2 ~> pf
-
-| rule_swap c pf : full_unf pf = swap -> (c _;_ Eps) <R= (Eps _;_ c) ~> pf (*New rule, from regex as types paper*)
-| rule_swapinv c pf : full_unf pf = swapinv -> (Eps _;_ c) <R= (c _;_ Eps) ~> pf
-
-| rule_proj c pf : full_unf pf = proj -> (Eps _;_ c) <R= c ~> pf
-| rule_projinv c pf : full_unf pf = projinv -> c <R=(Eps _;_ c) ~> pf
-
-| rule_abortR c pf : full_unf pf = abortR ->  c _;_ Empt <R= Empt ~> pf
-| rule_abortRinv c pf : full_unf pf = abortRinv ->  Empt  <R= c _;_ Empt ~> pf
-
-| rule_abortL c pf : full_unf pf = abortL -> Empt _;_ c <R=  Empt ~> pf
-| rule_abortLinv c pf : full_unf pf = abortLinv -> Empt  <R=  Empt _;_ c ~> pf
-
-| rule_distL c0 c1 c2 pf : full_unf pf = distL -> c0 _;_ (c1 _+_ c2) <R= (c0 _;_ c1) _+_ (c0 _;_ c2) ~> pf
-| rule_distLinv c0 c1 c2 pf : full_unf pf = distLinv -> (c0 _;_ c1) _+_ (c0 _;_ c2)  <R=  c0 _;_ (c1 _+_ c2) ~> pf
-
-| rule_distR c0 c1 c2 pf : full_unf pf = distR -> (c0 _+_ c1) _;_ c2 <R= (c0 _;_ c2) _+_ (c1 _;_ c2) ~> pf
-| rule_distRinv c0 c1 c2 pf : full_unf pf = distRinv ->  (c0 _;_ c2) _+_ (c1 _;_ c2)  <R= (c0 _+_ c1) _;_ c2 ~> pf
-
-
-| rule_wrap c pf : full_unf pf = wrap ->  Eps _+_ (c _;_ Star c) <R= Star c ~> pf
-| rule_wrapinv c pf : full_unf pf = wrapinv -> Star c  <R=Eps _+_ (c _;_ Star c) ~> pf
-
-| rule_drop c pf : full_unf pf = drop ->  Star (Eps _+_ c) <R= Star c ~> pf
-| rule_dropinv c pf : full_unf pf = dropinv ->  Star c <R= Star (Eps _+_ c) ~> pf (*Possibly redundant*)
-
- (*We want to remove inner Eps, so we only keep this one for now*)
-(*Will the other direction be necessary?*)
-(*| ci_star_plus_inv c :  Star c  <R= Star (Eps _+_ c) (*Could possibly be removed but we are studying the computational interpretation of EQ rules*) *)
-
-| rule_cid c pf : full_unf pf = cid ->  c <R= c ~> pf
-
-(*| ci_sym c0 c1 (H: c0 =R=c1) : c1 =R=c0*)
-| rule_ctrans c0 c1 c2 pf p0 p1 : full_unf pf =  ctrans p0 p1 ->  c0 <R=c1 ~> p0 ->  c1 <R=c2 ~> p1 -> c0 <R=c2 ~> pf
-| rule_cplus c0 c0' c1 c1' pf p0 p1 : full_unf pf = cplus p0 p1 ->  c0 <R=c0' ~> p0 -> c1 <R=c1' ~> p1 -> c0 _+_ c1 <R=c0' _+_ c1' ~> pf
-| rule_cseq c0 c0' c1 c1' pf p0 p1 : full_unf pf = cseq p0 p1 ->  c0 <R=c0' ~> p0 -> c1 <R=c1' ~> p1 ->  c0 _;_ c1 <R=c0' _;_ c1' ~> pf
-| rule_cstar c0 c1 pf p : full_unf pf = cstar p ->  c0 <R=c1 ~> p -> Star c0 <R= Star c1 ~> pf  (*new context rule*) 
-(*| rule_cfix r r' (p  : dsl) : r <R= r' ~> p[d (cfix p) .: var_dsl] ->  r <R= r' ~> (cfix p) (*guarded p otherwise unsound*)*)
-| rule_test a r r' pf p : full_unf pf = guard p -> P r r' p -> (Event a) _;_ r <R= (Event a) _;_ r' ~> pf
- where "c1 <R= c2 ~> p" := (c_ineq c1 c2 p).
-
-End Containment.
-
-
-Notation "c0 < ( R ) = c1 ~> p" := (c_ineq R c0 c1 p)(at level 63).
-Definition INEQ c0 c1 p := paco3 c_ineq bot3 c0 c1 p.
-Notation "c0 <C= c1 ~> p" := (INEQ c0 c1 p)(at level 63).
 
 (*Set Implicit Arguments.
 Unset Strict Implicit.
@@ -1562,276 +3022,6 @@ Unset Printing Implicit Defensive.*)
 
 
 
-
-
-
-Fixpoint interp (r0 r1 : regex)
-           (d : dsl2 dsl_co r0 r1)  (f : forall x y, dsl_co x y -> x <O= y ) :  r0 <O= r1 :=
-match d in dsl2 _ r0 r1 return (pTree r0) -> option (pTree r1) with 
-| @cid2 _ A => (@cid_o A)
-| @shuffle2 _ A B C => (@shuffle_o A B C)
-| @shuffleinv2 _ A B C => (@shuffleinv_o A B C)
-| @ctrans2 _ A B C d0 d1 => (@ctrans_o A B C) (@interp _ _ d0 f) (@interp _ _ d1 f)
-| @cplus2 _ A B C D d0 d1 => (@cplus_o A B C D (@interp _ _ d0 f)) (@interp _ _ d1 f)
-| @guard2 _ a A B pco => guard_o (f _ _ pco)
-end.
-
-Fixpoint interp_wrap (n : nat) (r0 r1 : regex) (d : dsl_co r0 r1) : r0 <O= r1 :=
-match d in dsl_co x y return x <O= y  with 
-          | Co_build _ _ dco => if n is n'.+1 then interp dco (interp_wrap n') else fun _ => None
-end. 
-
-
-
-Lemma fix_eq : forall n, ((fix interp_wrap (n0 : fin) (r0 r1 : regex) (d0 : dsl_co r0 r1) {struct n0} : r0 <O= r1 := match d0 in (dsl_co x y) return (x <O= y) with
-                                                                                                | @Co_build A1 B0 dco => match n0 with
-                                                                                                                         | 0 => fun=> None
-                                                                                                                         | n'.+1 => interp dco (interp_wrap n')
-                                                                                                                         end
-                                                                                                end) n) = interp_wrap n.
-Proof. done. Qed.
-
-Lemma interp_wrap_unf : forall n r0 r1 (d : dsl_co r0 r1), interp_wrap n.+1 d = match d in dsl_co x y return x <O= y  with 
-          | Co_build _ _ dco => interp dco (interp_wrap n) end.
-Proof. move => n r0 r1 d //=. 
-Qed.
-
-(*Require Import Coq.Program.Equality.*)
-(*Check interp.
-Lemma interp_wrap0 : forall r0 r1 (d : dsl2 dsl_co r0 r1), interp d (interp_wrap 0) = fun _ => None.
-Proof.
-move => r0 r1 d. fext. move=> x. 
-elim: d x=>//.
-rewrite /interp_wrap. case: d=>//.
-Qed.*)
-
-Lemma interp_trans : forall r0 r1 r2  (f : forall x y, dsl_co x y -> x <O= y) (d : dsl2 dsl_co r0 r1) (d' : dsl2 dsl_co r1 r2) T, interp (ctrans2 d d') f T -> interp d f T.
-Proof.
-move=> r0 r1 r2 f d d' T. rewrite /= /ctrans_o /obind /oapp /=. case: (interp _ _ _)=>//.
-Qed.
-
-
-Lemma interp_trans2 : forall r0 r1 r2  (f : forall x y, dsl_co x y -> x <O= y)  (d : dsl2 dsl_co r0 r1) (d' : dsl2 dsl_co r1 r2) T T', interp (ctrans2 d d') f T -> interp d f T = Some T' -> interp d' f T'.
-Proof.
-move => r0 r1 r2 Hf d d' T T' /= + Hsome. rewrite /= /ctrans_o /obind /oapp /=. rewrite Hsome //.
-Qed.
-
-Lemma pTree_eq : forall (A0 : regex), (fix pTree (r : regex) : Type := match r with
-                                           | Eps => unit
-                                           | Empt => void
-                                           | Event a => {a' : A & a' == a}
-                                           | r0 _+_ r1 => (pTree r0 + pTree r1)%type
-                                           | r0 _;_ r1 => (pTree r0 * pTree r1)%type
-                                           | Star r0 => seq (pTree r0)
-                                           end) A0 = pTree A0.
-Proof. done. Qed.
-
-Lemma reg_size1 : forall a (T : pTree (Event a)), @reg_size (Event a) T = 1.
-Proof.
-move=> a T. rewrite /reg_size //.
-Qed.
-
-Lemma interp_ineq : forall A B (d : dsl2 dsl_co A B) (T : pTree A) (T' : pTree B) (f : forall x y, dsl_co x y -> x <O= y), (forall x y (dco : dsl_co x y) (T0 : pTree x) (T1 : pTree y) , f x y dco T0 = Some T1 -> reg_size T1 <= reg_size T0) ->  
-                                                                                                                    interp d f T = Some T' -> reg_size T' <= reg_size T.
-Proof.
-move=> A' B d T T' f Hf.  
-- elim: d T T'.
- *  move=> B0 T0 T1 /=. rewrite /cid_o. case=>//->//.
- * move => A0 B0 C T T' /=. rewrite /shuffle_o /shuffle_i /=. case=><-. case: T=>//. by case.
- * move=> A0 B0 C T T' /=. rewrite /shuffleinv_o /shuffleinv_i /=. case=><-. case: T=>//. by case.
- * move=> A0 B0 C d IH d0 IH2 T T' Hsome. 
-   have: interp (ctrans2 d d0) f T by rewrite Hsome//. 
-   move/[dup]=>Tsome. move/interp_trans.
-   case Heq: (interp _ _ _)=>// [T''] _. move: (IH _ _ Heq)=>Hsize. 
-   move/interp_trans2: (Heq). move/(_ _ d0 Tsome).
-   case Heq2: (interp _ _ _)=>// [T'''] _. move: (IH2 _ _ Heq2). 
-   move=> Hsize2.
-   move: Hsome. rewrite /= /ctrans_o /= /obind /oapp /= Heq Heq2.
-   case. move=> HT;subst. lia.
- * move=> A0 B0 C D d IH d0. move=> IH2 T T' /=. rewrite /cplus_o /=. 
-   case: T. 
-  **  move=> T2. rewrite /omap /obind /oapp. 
-      case Heq: (interp _ _ _) => // [T3 ]. case. move=> HT3;subst. apply/IH. eauto. 
-  **  move=> T2. rewrite /omap /obind /oapp. 
-      case Heq: (interp _ _ _) => // [T3 ]. case. move=> HT3;subst. apply/IH2. eauto. 
- * move => A0 B0 r T T' /= T'0. rewrite /guard_o. destruct T' eqn:Heqn. subst. destruct (f _ _ _ _) eqn:Heqn. case. move=> Ht0;subst. 
-   suff: reg_size a1 <= reg_size a0. lia.  eauto. done.
-Qed.
-Check interp_wrap.
-Lemma interp_wrap_ineq : forall n A B (d : dsl_co A B) (T : pTree A) (T' : pTree B),  interp_wrap n d T = Some T' -> reg_size T' <= reg_size T.
-Proof.
-elim.
-- move=> A0 B [] //=.
-- move=> n IH A0 B [] T T' d T0 T0'. rewrite interp_wrap_unf. move=> Hint.  apply/interp_ineq;last by eauto. 
-  move=> x y dco T1 T2 Hin. eauto.
-Qed.
-
-
-Lemma interp_some : forall A B (f : forall x y, dsl_co x y -> x <O= y) (d : dsl2 dsl_co A B) (T : pTree A) , (forall x y (dco : dsl_co x y) (T0 : pTree x), f x y dco T0) ->  
-                                                                                                                    interp d f T.
-Proof.
-move=> A' B f. 
-- elim=>//. 
-(* *  move=> B0 T0 T1 /=. rewrite /cid_o. case=>//->//.
- * move => A0 B0 C T T' /=. rewrite /shuffle_o /shuffle_i /=. case=><-. case: T=>//. by case.
- * move=> A0 B0 C T T' /=. rewrite /shuffleinv_o /shuffleinv_i /=. case=><-. case: T=>//. by case.*)
- * move=> A0 B0 C d IH d0 IH2 T Hf. 
-   rewrite /= /ctrans_o /obind /oapp /=.
-   move: (@IH T Hf). case Hcase: (interp _ _ _)=>// [T1] _.
-   apply/IH2. eauto.
- * move=> A0 B0 C D d IH d0. move=> IH2 T Hf /=. rewrite /cplus_o /=. 
-   case: T. 
-  **  move=> T2. rewrite /omap /obind /oapp. 
-      move: (@IH T2 Hf).
-      case Heq: (interp _ _ _) => // [T3 ]. 
-  **  move=> T2. rewrite /omap /obind /oapp. 
-      move: (@IH2 T2 Hf).
-      case Heq: (interp _ _ _) => // [T3 ]. 
- * move => A0 B0 C r T Hf /=. rewrite /guard_o. destruct T eqn:Heqn;subst.
-   move: (Hf B0 C r a0). case: (f _ _ _)=>//.
-Qed.
-
-
-(*Lemma interp_ineq : forall A B (d : dsl2 dsl_co A B) (T : pTree A) (T' : pTree B) n, interp d (interp_wrap n) T = Some T' -> reg_size T' <= reg_size T.
-Proof.
-move=> A' B. 
-- elim=>//.
- *  move=> B0 T0 T1 _ /=. rewrite /cid_o. case=>//->//.
- * move => A0 B0 C T T' _ /=. rewrite /shuffle_o /shuffle_i /=. case=><-. case: T=>//. by case.
- * move=> A0 B0 C T T' _ /=. rewrite /shuffleinv_o /shuffleinv_i /=. case=><-. case: T=>//. by case.
- * move=> A0 B0 C d IH d0 IH2 T T' n Hsome. 
-   have: interp (ctrans2 d d0) (interp_wrap n) T by rewrite Hsome//. 
-   move/[dup]=>Tsome. move/interp_trans.
-   case Heq: (interp _ _ _)=>// [T''] _. move: (IH _ _ _ Heq)=>Hsize. 
-   move/interp_trans2: (Heq). move/(_ _ d0 Tsome).
-   case Heq2: (interp _ _ _)=>// [T'''] _. move: (IH2 _ _ _ Heq2). 
-   move=> Hsize2.
-   move: Hsome. rewrite /= /ctrans_o /= /obind /oapp /= Heq Heq2.
-   case. move=> HT;subst. lia.
- * move=> A0 B0 C D d IH d0. move=> IH2 T T'  n/=. rewrite /cplus_o /=. 
-   case: T. 
-  **  move=> T2. rewrite /omap /obind /oapp. 
-      case Heq: (interp _ _ _) => // [T3 ]. case. move=> HT3;subst. apply/IH. eauto. 
-  **  move=> T2. rewrite /omap /obind /oapp. 
-      case Heq: (interp _ _ _) => // [T3 ]. case. move=> HT3;subst. apply/IH2. eauto. 
- * move => A0 B0 r T T' /=.  destruct r=>//.
-- move=> n IH d T T'. rewrite /=. 
-*)
-
-(*Lemma interp_ineq : forall A B n (d : dsl2 dsl_co A B) (T : pTree A) (T' : pTree B), interp d (interp_wrap n) T = Some T' -> reg_size T' <= reg_size T.
-Proof.
-move=> A' B. elim=>//.
-- move=> d T T'. 
-  elim: d T T'=>//.
- *  move=> B0 T0 T1 /=. rewrite /cid_o. case=>//->//.
- * move => A0 B0 C T T' /=. rewrite /shuffle_o /shuffle_i /=. case=><-. case: T=>//. by case.
- * move=> A0 B0 C T T' /=. rewrite /shuffleinv_o /shuffleinv_i /=. case=><-. case: T=>//. by case.
- * move=> A0 B0 C d IH d0 IH2 T T' Hsome. 
-   have: interp (ctrans2 d d0) (interp_wrap 0) T by rewrite Hsome//. 
-   move/[dup]=>Tsome. move/interp_trans.
-   case Heq: (interp _ _ _)=>// [T''] _. move: (IH _ _ Heq)=>Hsize. 
-   move/interp_trans2: (Heq). move/(_ _ d0 Tsome).
-   case Heq2: (interp _ _ _)=>// [T'''] _. move: (IH2 _ _ Heq2). 
-   move=> Hsize2.
-   move: Hsome. rewrite /= /ctrans_o /= /obind /oapp /= Heq Heq2.
-   case. move=> HT;subst. lia.
- * move=> A0 B0 C D d IH d0. move=> IH2 T T' /=. rewrite /cplus_o /=. 
-   case: T. 
-  **  move=> T2. rewrite /omap /obind /oapp. 
-      case Heq: (interp _ _ _) => // [T3 ]. case. move=> HT3;subst. apply/IH. done.
-  **  move=> T2. rewrite /omap /obind /oapp. 
-      case Heq: (interp _ _ _) => // [T3 ]. case. move=> HT3;subst. apply/IH2. done.
- * move => A0 B0 r T T' /=.  destruct r=>//.
-- move=> n IH d T T'. rewrite /=. 
-
-case Hcase: (interp _ _ _)=>// [T2]. case=>HT2;subst.
-  apply/IH.  eauto.
-move => Hin. apply/IH.
- case Hcase: r.
-  **
-rewrite fix_eq.
- move.
-lia.
- Tsome).
-   move: (interp_trans2 _ _ _ _ _ _ _ _ Tsome Heq).
-
-   
-suff: reg_size T <= reg_size T'' by lia.
-move/[dup]. move/interp_transp.
-   rewrite /interp.
-C T T' /=. rewrite /shuffleinv_o /shuffleinv_i /=. case=><-. case: T=>//. by case.
-
- rewrite /shuffle_i //. 
-   move
-destruct T,T';ssa. destruct a;ssa.
- case: T=>//.
-rewrite interp_wrap0.
-
-d T T' n Hsome.
- pTree A1
-  Hsize : reg_size A1 T < n.+1
-  T' : pTree B0
-  Heq : interp d (interp_wrap n) T = Some T'
-*)
-
-(*Lemma interp_wrap_some : forall n r0 r1 (d : dsl_co r0 r1) (T : pTree r0), reg_size T < n -> { T' | interp_wrap n d T = Some T'}.
-Proof.
-elim.
-- move=> r0 r1 d T // Hsize.  
-- move => n IH r0 r1 d T Hsize /=. destruct d.
-  elim: d T Hsize IH=>//.
- * move=> B0 T Hsize IH. 
- move=> B0. C d IH d0 IH2 T Hsize IH3 /=. rewrite /ctrans_o /obind /oapp /=.
-   have: interp d (interp_wrap n) T;first by eauto. case Hcase: (interp _ _ _)=>// [ T1 ] _.
-   apply/IH2.
-   have : reg_size T1 <= reg_size T by 
-   apply/interp_ineq;last eauto; move=> x y dco T0 T2 Hint; apply/interp_wrap_ineq; eauto.
-   move=> Hsize2. lia.
- * move=> r0 r1 d1 T0. eauto.
- * move=> A1 B0 C D d IH d0 IH1 T Hsize IH2 /=. rewrite /cplus_o.
-   destruct T; rewrite /omap /obind /oapp.
-   have: interp d (interp_wrap n) a. eauto. case Hcase: (interp _ _ _)=>//.
-   rewrite /omap /obind /oapp.
-   have: interp d0 (interp_wrap n) a. eauto. case Hcase: (interp _ _ _)=>//.
- * move=> a B0 C r T Hsize IH /=. rewrite /guard_o. destruct T.
-   have: (interp_wrap n r a1). by eauto. case: (interp_wrap _ _ _)=>//.
-Qed.*)
-
-Lemma interp_wrap_some : forall n r0 r1 (d : dsl_co r0 r1) (T : pTree r0), reg_size T < n -> interp_wrap n d T.
-Proof.
-elim.
-- move=> r0 r1 d T // Hsize.  
-- move => n IH r0 r1 d T Hsize /=. destruct d.
-  elim: d T Hsize IH=>//.
- * move=> A1 B0 C d IH d0 IH2 T Hsize IH3 /=. rewrite /ctrans_o /obind /oapp /=.
-   have: interp d (interp_wrap n) T;first by eauto. case Hcase: (interp _ _ _)=>// [ T1 ] _.
-   apply/IH2.
-   have : reg_size T1 <= reg_size T by 
-   apply/interp_ineq;last eauto; move=> x y dco T0 T2 Hint; apply/interp_wrap_ineq; eauto.
-   move=> Hsize2. lia.
- * move=> r0 r1 d1 T0. eauto.
- * move=> A1 B0 C D d IH d0 IH1 T Hsize IH2 /=. rewrite /cplus_o.
-   destruct T; rewrite /omap /obind /oapp.
-   have: interp d (interp_wrap n) a. eauto. case Hcase: (interp _ _ _)=>//.
-   rewrite /omap /obind /oapp.
-   have: interp d0 (interp_wrap n) a. eauto. case Hcase: (interp _ _ _)=>//.
- * move=> a B0 C r T Hsize IH /=. rewrite /guard_o. destruct T.
-   have: (interp_wrap n r a1). by eauto. case: (interp_wrap _ _ _)=>//.
-Qed.
-
-Lemma interp_wrap_sig : forall n r0 r1 (d : dsl_co r0 r1) (T : pTree r0), reg_size T < n -> { T' | interp_wrap n d T = Some T'}.
-Proof.
-move=> n r0 r1 d T Hsize.
-move: (interp_wrap_some  n d T Hsize). case Hcase: (interp_wrap n d T)=>// [T'] _. econ. eauto.
-Qed.
-
-Lemma size_proof : forall (r : regex) (T : pTree r), leq ((reg_size T)) (reg_size T). done. Defined.
-
-Definition interp_total (r0 r1 : regex) (d : dsl_co r0 r1) := 
-fun T =>
-match interp_wrap_sig (reg_size T).+1 d T (size_proof r0 T) with
-| exist T' _ => T'
-end.
 
 
 
