theories/dsl_theory.v
@@ -1,0 +1,113 @@
+From mathcomp Require Import all_ssreflect zify.
+Require Import Containment.dsl.
+Set Implicit Arguments.
+Unset Strict Implicit.
+Unset Printing Implicit Defensive.
+
+Require Import Containment.utils.
+
+
+(*Adapted from a development on session types*)
+Fixpoint mu_height g :=
+match g with
+| cfix l => (mu_height l).+1
+| _ => 0
+end.
+
+Definition unf g := if g is cfix g' then g' [d g .: var_dsl]  else g.
+Definition full_unf g := (iter (mu_height g) unf g).
+
+
+(*guarded in the sense that full_unf d <> cfix ... 
+  It might still be a non-terminating program (cfix. shuffle (var 0))
+*)
+Fixpoint guarded (i : nat) d := 
+match d with
+| var_dsl j => j != i
+| cfix d' => guarded i.+1 d'
+| _ => true 
+end. 
+Print dsl.
+Fixpoint contractive d := 
+match d with
+| cfix d' => (guarded 0 d') && (contractive d')
+| ctrans d0 d1 => (contractive d0) && (contractive d1)
+| cplus d0 d1 => (contractive d0) && (contractive d1)
+| cseq d0 d1 => (contractive d0) && (contractive d1)
+| cstar d0 => (contractive d0)
+| guard d0 => (contractive d0)
+| _ => true 
+end. 
+
+
+
+
+
+Lemma mu_height_ren : forall g sigma, mu_height g ⟨d sigma ⟩  = mu_height g.
+Proof.
+elim;rewrite /=;try done;intros.
+f_equal. apply : H. 
+Qed.
+
+Lemma mu_height_subst : forall g0 sigma, (forall n, ~~ guarded n g0 -> mu_height (sigma n) = 0) ->  mu_height (g0[d sigma]) = mu_height g0.
+Proof. 
+elim; try solve [by rewrite /=];intros.
+asimpl. move : (H n). destruct (mu_height (sigma n)) eqn:Heqn. done. have : 0 < n0.+1 by lia. move => + HH. simpl. 
+simpl in HH. lia. 
+simpl. f_equal. asimpl. apply H. case. done.  simpl. intros. asimpl. rewrite mu_height_ren. apply/H0. done. 
+Qed.
+
+
+Lemma mu_height_unf : forall g , guarded 0 g -> (mu_height g) = mu_height (g [d cfix g .: var_dsl]).
+Proof.
+move => g. rewrite /=. case : g; try solve [intros;rewrite /=;done].
+intros. rewrite /=. destruct n. done. done. ssa. erewrite mu_height_subst. done. case. done. 
+intros. simpl. asimpl. destruct n. lia.  simpl. done. 
+Qed.
+
+Lemma mu_height_unf2 : forall g sigma i, ~~ guarded i g -> (mu_height g) + mu_height (sigma i) = mu_height (g [d sigma]).
+Proof. 
+elim;rewrite //=;intros. have : n = i by lia.  intros. subst. lia. 
+asimpl. erewrite <- H. 2 : { eauto. } simpl. asimpl. rewrite mu_height_ren. lia. 
+Qed.
+
+
+Lemma guarded_test : forall e sigma i,  ~~ guarded i e -> iter (mu_height e) unf e [d sigma ] = sigma i. 
+Proof. 
+elim;rewrite //=;intros. 
+have : n = i. lia.  move=>->. done.  asimpl. rewrite -iterS iterSr. simpl. asimpl. erewrite H. 
+2 : { eauto. } simpl. done. 
+Qed.
+
+
+(*Even non contractive terms have the property that full unfolding equals full unfolding plus 1. This is what we need in projection lemma
+ so we don't have to derive contractiveness of e from projection derivation*)
+Lemma full_unf_subst : forall e, full_unf (cfix e) = full_unf (e [d cfix e .: var_dsl]). 
+Proof. 
+intros. rewrite /full_unf. 
+intros. simpl.  rewrite -iterS iterSr. simpl. 
+destruct (guarded 0 e) eqn:Heqn.  rewrite mu_height_unf. done. done. 
+ erewrite guarded_test.  2 : { lia. } 
+simpl. 
+erewrite <-mu_height_unf2. 2 : { lia.  } simpl. 
+rewrite addnC.  
+rewrite iterD. erewrite guarded_test. 2 : { lia.  } simpl. rewrite -iterS iterSr /=. 
+erewrite guarded_test. 2 : { lia. } done. 
+Qed.
+
+
+Lemma full_unf2 : forall n e, full_unf (iter n unf e) = full_unf e. 
+Proof. 
+elim. done. 
+intros. rewrite iterS. 
+destruct (if (iter n unf e) is cfix _ then true else false) eqn:Heqn. 
+destruct ((iter n unf e))eqn:Heqn2;try done. simpl. 
+rewrite -(H e) Heqn2. rewrite full_unf_subst. done. 
+have : unf (iter n unf e) = iter n unf e. destruct ((iter n unf e));try done. 
+move=>->. rewrite H. done. 
+Qed.
+
+Lemma full_unf_idemp : idemp full_unf. 
+Proof. 
+intros. rewrite /idemp. intros. rewrite {2}/full_unf. rewrite full_unf2. done. 
+Qed.
